clean elpi

code/rocq/elpi.v
@@ -17,13 +17,23 @@ Module Nur (U : Unif).
 
   Module VS := valid_state(U).
   Import VS RunP Run Language.
+  Lemma same_subst (s1 s2: Sigma): s1 = s2. Admitted.
   
+  (* The bool in the cut is to know if the cut is deep.
+     For expamle, in the state:
+      ((! \/ A) /\ !) \/ C
+    The first cut is deep, therefore its cut-to alternatives point to C
+    The second cut is superficial, therfore its cut to alternatives are empty
+  *)
   Inductive G := 
     | call : program -> Tm -> G
-    | cut : bool -> list (list G) -> G (*the bool tells if it is a superficial cut*)
+    | cut : bool -> list (list G) -> G
     .
+
   (* derive G. *)
   (* HB.instance Definition _ := hasDecEq.Build G G_eqb_OK. *)
+  Definition is_cut' A := match A with cut _ _ => true | _ => false end.
+  Definition cuts' A := all is_cut' A.
 
   Definition alt := (list G).
 
@@ -36,13 +46,31 @@ Module Nur (U : Unif).
   Definition trad_prems p (b : Sigma * R) :=
     map (trad p) b.2.(premises).
 
-  Definition add_ca alts a :=
-    match a with
-    | cut lvl a1 => cut lvl (a1 ++ alts)
-    | call pr t => call pr t
-    end.
+  Section add_ca.
 
-  Definition save_alt a gs b := map (add_ca a) b ++ gs.
+    Definition add_ca always alts a := (*always:= adds always alts to cut *)
+      match a with
+      | cut lvl a1 => if always || lvl then cut lvl (a1 ++ alts) else a
+      | call pr t => call pr t
+      end.
+
+    Lemma add_ca_empty {b lA}:
+      map (add_ca b [::]) lA = lA.
+    Proof.
+      rewrite /add_ca; elim: lA b => //= x xs IH b.
+      rewrite IH; case: x => //-[]// l; rewrite cats0//if_same//.
+    Qed.
+
+    Lemma map_add0_cas_empty {lA b}:
+      map (map (add_ca b [::])) lA  = lA.
+    Proof.
+      rewrite /add_ca; elim: lA => //= x xs ->.
+      f_equal; apply add_ca_empty.
+    Qed.
+  End add_ca.
+
+
+  Definition save_alt a gs b := map (add_ca true a) b ++ gs.
   Definition more_alt a bs gs := map (save_alt a gs) bs ++ a.
 
   Inductive nur : Sigma -> list G ->  list alt -> Sigma -> list alt -> Prop :=
@@ -72,96 +100,66 @@ Module Nur (U : Unif).
       congruence.
   Qed.
 
-  Definition add_ca0 alts a :=
-    match a with
-    | cut true a1 => cut true a1
-    | cut false a1 => cut false (a1 ++ alts)
-    | call pr t => call pr t
-    end.
+  Section makers.
+    (* here we don't add the alts only to deep cut *)
+    Definition make_lB lB tl := map (map (add_ca false tl)) lB.
 
-  Lemma add_ca0_empty lA:
-    map (add_ca0 [::]) lA = lA.
-  Proof.
-    rewrite /add_ca0; elim: lA => //= x xs ->.
-    case: x => //-[]// l; rewrite cats0//.
-  Qed.
+    Lemma make_lB_empty1 {tl} : make_lB [::] tl = [::].
+    Proof. move=>//. Qed.
 
-  Lemma map_add0_cas_empty lA:
-    map (map (add_ca0 [::])) lA  = lA.
-  Proof.
-    rewrite /add_ca0; elim: lA => //= x xs ->.
-    f_equal; apply add_ca0_empty.
-  Qed.
+    Lemma make_lB_empty2 {lB} : make_lB lB [::] = lB.
+    Proof. rewrite/make_lB map_add0_cas_empty//. Qed.
 
-  Lemma add_ca_empty lA:
-    map (add_ca [::]) lA = lA.
-  Proof.
-    rewrite /add_ca; elim: lA => //= x xs ->.
-    case: x => //-[]// l; rewrite cats0//.
-  Qed.
+    Definition make_lB0 xs (lB0: list alt) := [seq la ++ lb | la <- xs, lb <- lB0].
 
-  Lemma map_add_cas_empty lA:
-    map (map (add_ca [::])) lA  = lA.
-  Proof.
-    rewrite /add_ca; elim: lA => //= x xs ->.
-    f_equal; apply add_ca_empty.
-  Qed.
+    Lemma make_lB0_empty1 {lb0} : make_lB0 [::] lb0 = [::].
+    Proof. rewrite /make_lB0//. Qed.
 
-  Definition make_lB lB tl := map (map (add_ca0 tl)) lB.
+    Lemma make_lB0_empty2 {xs} : make_lB0 xs [::] = [::].
+    Proof. rewrite /make_lB0/=flatten_empty//. Qed.
 
-  Lemma make_lB_empty1 {tl} : make_lB [::] tl = [::].
-  Proof. move=>//. Qed.
+    Definition add_alt x xs (lB0 lB:list alt) : list  alt :=
+      let: lB := make_lB lB (make_lB0 xs lB0) in
+      [seq x ++ y | y <- lB] ++ (make_lB0 xs lB0).
 
-  Lemma make_lB_empty2 {lB} : make_lB lB [::] = lB.
-  Proof. rewrite/make_lB map_add0_cas_empty//. Qed.
+    Lemma add_alt_empty1 {xs lB0 lB}:
+      add_alt [::] xs lB0 lB = (make_lB lB (make_lB0 xs lB0)) ++ (make_lB0 xs lB0).
+    Proof. rewrite /add_alt/=map_id//. Qed.
 
-  Definition make_lB0 xs (lB0: list alt) := [seq la ++ lb | la <- xs, lb <- lB0].
+    Lemma add_alt_empty2 {x lB0 lB}:
+      add_alt x [::] lB0 lB = [seq x ++ y | y <- lB].
+    Proof. rewrite/add_alt/=/make_lB cats0 map_add0_cas_empty//. Qed.
 
-  Lemma make_lB0_empty1 {lb0} : make_lB0 [::] lb0 = [::].
-  Proof. rewrite /make_lB0//. Qed.
+    Lemma add_alt_empty3 {x xs lB}:
+      add_alt x xs [::] lB = [seq x ++ y | y <- lB].
+    Proof. rewrite/add_alt !make_lB0_empty2 make_lB_empty2 cats0//. Qed.
 
-  Lemma make_lB0_empty2 {xs} : make_lB0 xs [::] = [::].
-  Proof. rewrite /make_lB0/=flatten_empty//. Qed.
+    Lemma add_alt_empty4 {x xs lB0}:
+      add_alt x xs lB0 [::] = make_lB0 xs lB0.
+    Proof. rewrite/add_alt/=/make_lB//. Qed.
+  End makers.
 
-  Definition add_alt x xs (lB0 lB:list alt) : list  alt :=
-    let: lB := make_lB lB (make_lB0 xs lB0) in
-    [seq x ++ y | y <- lB] ++ (make_lB0 xs lB0).
+  Section incr_cut.
+    Definition incr_cut A :=
+      match A with
+      | cut _ ca => cut true ca
+      | _ => A
+      end.
 
-  Lemma add_alt_empty1 {xs lB0 lB}:
-    add_alt [::] xs lB0 lB = (make_lB lB (make_lB0 xs lB0)) ++ (make_lB0 xs lB0).
-  Proof. rewrite /add_alt/=map_id//. Qed.
+    Definition incr_cuts := map (map incr_cut).
 
-  Lemma add_alt_empty2 {x lB0 lB}:
-    add_alt x [::] lB0 lB = [seq x ++ y | y <- lB].
-  Proof. rewrite/add_alt/=/make_lB cats0 map_add0_cas_empty//. Qed.
+    Lemma incr_cuts_cat {l1 l2}: incr_cuts (l1 ++ l2) = incr_cuts l1 ++ incr_cuts l2.
+    Proof. rewrite/incr_cuts map_cat//. Qed.
 
-  Lemma add_alt_empty3 {x xs lB}:
-    add_alt x xs [::] lB = [seq x ++ y | y <- lB].
-  Proof. rewrite/add_alt !make_lB0_empty2 make_lB_empty2 cats0//. Qed.
+    Lemma incr_cuts0 {l}: incr_cuts l = [::] -> l =[::].
+    Proof. case: l => //. Qed.
 
-  Lemma add_alt_empty4 {x xs lB0}:
-    add_alt x xs lB0 [::] = make_lB0 xs lB0.
-  Proof. rewrite/add_alt/=/make_lB//. Qed.
+    Lemma incr_cut2 {l}: map incr_cut (map incr_cut l) = map incr_cut l.
+    Proof. elim: l => // x xs /=->; case: x => //. Qed.
 
-  Definition incr_cut A :=
-    match A with
-    | cut _ ca => cut false ca
-    | _ => A
-    end.
-
-  Definition incr_cuts := map (map incr_cut).
-
-  Lemma incr_cuts_cat {l1 l2}: incr_cuts (l1 ++ l2) = incr_cuts l1 ++ incr_cuts l2.
-  Proof. rewrite/incr_cuts map_cat//. Qed.
-
-  Lemma incr_cuts0 {l}: incr_cuts l = [::] -> l =[::].
-  Proof. case: l => //. Qed.
-
-  Lemma incr_cut2 {l}: map incr_cut (map incr_cut l) = map incr_cut l.
-  Proof. elim: l => // x xs /=->; case: x => //. Qed.
-
-  Lemma incr_cuts2 {l}: incr_cuts (incr_cuts l) = incr_cuts l.
-  Proof. elim: l => // x xs /=->; rewrite incr_cut2//. Qed.
+    Lemma incr_cuts2 {l}: incr_cuts (incr_cuts l) = incr_cuts l.
+    Proof. elim: l => // x xs /=->; rewrite incr_cut2//. Qed.
+  End incr_cut.
 
   (* bt is the backtracking list for the cut-alternatives
      this list is important since in this tree:
@@ -183,13 +181,14 @@ Module Nur (U : Unif).
     | Top => [::[::]]
     | Bot => [::]
     | Dead => [::]
-    | Goal _ Cut => [::[::cut true [::]]]
+    | Goal _ Cut => [::[::cut false [::]]]
     | Goal pr (Call t) => [::[::call pr t]]
     | Or A _ B => 
       let lB := state_to_list B bt in
       let lA := state_to_list A (lB ++ bt) in
       (* here we are adding bt to lA. In the example above J in not in bt  *)
-      incr_cuts (map (map (add_ca bt)) lA ++ lB)
+      (* since bt are at least grand-parents alts, then we force the insertion in the cuts of lA *)
+      incr_cuts (map (map (add_ca true bt)) lA ++ lB)
     | And A B0 B =>
       let lA   := state_to_list A bt in
       let lB   := state_to_list B bt in
@@ -240,11 +239,12 @@ Module Nur (U : Unif).
     Qed.
 
     Goal forall p a b s1 s2, 
+    (* (! \/ a) \/ b *)
       state_to_list (
         Or 
           (Or (Goal p Cut) s1 (Goal p (Call a))) s2
           (Goal p (Call b))) [::] = 
-      [:: [:: cut false [:: [:: call p b]]]; [:: call p a]; [:: call p b]].
+      [:: [:: cut true [:: [:: call p b]]]; [:: call p a]; [:: call p b]].
     Proof. by []. Qed.
 
     Goal forall A1 A2 s  C0 B p,
@@ -270,14 +270,14 @@ Module Nur (U : Unif).
         Or 
           (Or (And (Goal p (Call c)) b0 (Goal p Cut)) s1 (Goal p (Call a))) s2
           (Goal p (Call b))) [::] = 
-      [:: [:: call p c; cut false [:: [:: call p b]]]; [:: call p a]; [:: call p b]].
+      [:: [:: call p c; cut true [:: [:: call p b]]]; [:: call p a]; [:: call p b]].
     Proof. by []. Qed.
 
     Goal forall s1 s2 B C Res p,
       let f x := (Goal p (Call x)) in
       (* (OK \/ B) /\ (! \/ C) -> [cut_[B,Reset]; C; (B, Reset)] *)
       state_to_list (And (Or OK s1 (f B)) (f Res) (Or (Goal p Cut) s2 (f C))) [::]
-        = [::[::cut false [::[:: call p B; call p Res]]]; [::call p C]; [:: call p B; call p Res]].
+        = [::[::cut true [::[:: call p B; call p Res]]]; [::call p C]; [:: call p B; call p Res]].
     Proof.
       move=> s1 s2 B C Res p//=.
     Qed.
@@ -286,7 +286,7 @@ Module Nur (U : Unif).
       let f x := (Goal p (Call x)) in
       (* (OK \/ B) /\ (! /\ C) -> [cut_[]; C; (B, Reset)] *)
       state_to_list (And (Or OK s1 (f B)) (f Res) (And (Goal p Cut) (f Res2) (f C))) [::]
-        = [::[::cut true [::]; call p C]; [:: call p B; call p Res]].
+        = [::[::cut false [::]; call p C]; [:: call p B; call p Res]].
     Proof.
       move=> s1 B C Res Res2 p//=.
     Qed.
@@ -296,7 +296,7 @@ Module Nur (U : Unif).
       (* (A /\ ((! \/ B) \/ C) *)
       state_to_list (And (f A) (f C0) (Or (Or (Goal p Cut) s1 (f B)) s2 (f C))) [::]
       = [:: 
-        [:: call p A; cut false [:: [:: call p C]]]; 
+        [:: call p A; cut true [:: [:: call p C]]]; 
         [:: call p A; call p B]; 
         [:: call p A; call p C]].
     Proof.
@@ -309,7 +309,7 @@ Module Nur (U : Unif).
       state_to_list 
         (And (Or (f A) s1 (f B)) (f C) (Or (Or (Goal p Cut) s2 (f D)) s3 (f E))) [::] = 
         [:: 
-        [:: call p A; cut false [:: [:: call p E]; [:: call p B; call p C]]];
+        [:: call p A; cut true [:: [:: call p E]; [:: call p B; call p C]]];
         [:: call p A; call p D]; [:: call p A; call p E];
         [:: call p B; call p C]]
       .
@@ -324,7 +324,7 @@ Module Nur (U : Unif).
       state_to_list 
         (And (Or (f A) s1 (f B)) (f C) (And (Or (Goal p Cut) s2 (f D)) (f E) (f F))) [::] = 
         [:: 
-          [:: call p A; cut false [:: [:: call p B; call p C]]; call p F];
+          [:: call p A; cut true [:: [:: call p B; call p C]]; call p F];
           [:: call p A; call p D; call p E]; 
           [:: call p B; call p C]].
     Proof.
@@ -345,7 +345,7 @@ Module Nur (U : Unif).
       state_to_list 
         (And (Or (f A) s1 (f B)) (f C) (And (Or (Goal p Cut) s2 (f D)) (f E) (Goal p Cut))) [::] = 
         [:: 
-          [:: call p A; cut false [:: [:: call p B; call p C]]; cut true [::]];
+          [:: call p A; cut true [:: [:: call p B; call p C]]; cut false [::]];
           [:: call p A; call p D; call p E]; 
           [:: call p B; call p C]].
     Proof.
@@ -398,6 +398,8 @@ Module Nur (U : Unif).
       next_alt s3 (big_and p l) = Some (s3, (big_and p l)).
     Proof. elim: l p s3 => //; move=> a l IH p s3 => /=; rewrite IH//. Qed.
 
+    Ltac madmit := admit.
+
     Goal forall s1 s2 B C D E p,
       let f x := (Goal p (Call x)) in
       (* (A \/_{s1} B) /\_C ((! \/_{s2} D) /\_{E} F) *) 
@@ -446,7 +448,7 @@ Module Nur (U : Unif).
                 - move=> [??]; subst; inversion_clear H5; subst => //.
                   move: H0 => /=[?]; subst => //.
                 - move=>[??]; subst.
-                  (have ?: s' = s'0 by admit); subst.
+                  have:= (same_subst s' s'0); move=> ?; subst.
                   apply: CallE f1 _.
                   move=> /=.
                   inversion_clear H5; subst => //.
@@ -477,50 +479,176 @@ Module Nur (U : Unif).
                         inversion_clear H3; subst => //.
                         move: H0 => /=[??]; subst.
                         inversion_clear H5; subst => //; move: H0 => /=; rewrite /big_or; case f1: F => [|[s4 r1] rs1]//=-[?]; subst => //.
-                        (have ?: s' = s'0 by admit); subst.
+                        (have ?: s' = s'0 by apply same_subst); subst.
                         apply: CallE f1 _.
                         rewrite/more_alt/save_alt/=cats0.
                         move: H2; case: rs1 => [|[s6 r2] rs1]//=.
                         - rewrite is_dead_big_and next_alt_big_and.
                           move=>[??]; subst.
-                          admit.
+                          madmit.
                         - rewrite is_dead_big_and/=next_alt_big_and => -[??]; subst.
-                          admit.
-                    - admit.
+                          madmit.
+                    - madmit.
                   - move=> [s4 r1] l/=; rewrite is_dead_big_and next_alt_big_and.
                     move=> [??]; subst.
                     rewrite /more_alt/save_alt/=.
-                    admit.
+                    madmit.
           - move=>[?]; subst.
             rewrite /=is_dead_big_or in H3.
             apply: CallE .
-            (* (have ?: s' = s'0 by admit); subst.
-            case : r1. *)
         -
         -
     Abort.
 
   End tests.
 
-  (* Lemma base_and_propagate_cut {A}:
-    base_and A -> propagate_cut A.
-  Proof. elim: A => // -[]//= _ _ _ ? _ ? H/andP[_]/H->//. Qed. *)
+  (* superficial cut *)
+  Section lvlS.
+    Definition lvlS A:= match A with cut b1 _ => ~~b1 | _ => true end.
 
+    Lemma base_and_state_to_list {A}: base_and A -> exists hd, forall l, state_to_list A l = [::hd].
+    Proof.
+      elim: A => //.
+      - by eexists.
+      - move=> []//p a _ B0 _ B HB/=/andP[/eqP->bB].
+        have [hd H]/= := HB bB.
+        case: a => [|t]; eexists => l; rewrite H //.
+    Qed.
+
+    Lemma base_and_lvlt {A l hd}: 
+      base_and A -> state_to_list A l = [::hd] -> all lvlS hd.
+    Proof.
+      elim: A l hd => //.
+      - move=> l hd _ [<-]//.
+      - move=> []// p a _ B0 _ B HB l hd/=/andP[/eqP->bB].
+        have [hd1 H]:= base_and_state_to_list bB; rewrite H.
+        case: a => //[|t]; rewrite add_alt_empty2/==>-[?]; subst => /=; apply: HB bB (H [::]).
+    Qed.
+
+    Lemma lvlt_add_caF {y l}:
+      lvlS y -> add_ca false l y = y.
+    Proof. case: y => //-[]//l1/=. Qed.
+
+    Lemma all_lvlt_add_caF {y l}:
+      all lvlS y -> [seq add_ca false l e | e <- y] = y.
+    Proof.
+      elim: y l => //=x xs IH l/andP[lx lxs].
+      rewrite IH//lvlt_add_caF//.
+    Qed.
+  End lvlS.
+
+  (* deep cut *)
+  Section lvlD.
+    Definition lvlD A := match A with cut b1 _ => b1 | _ => true end.
+
+    Lemma lvlF_incr {x}: lvlD x -> incr_cut x = x.
+    Proof. case: x => //-[]//. Qed.
+
+    Lemma all_lvlF_incr {ca}:
+      all lvlD ca -> map incr_cut ca = ca.
+    Proof. elim: ca => //x xs IH/=/andP[H1 H2]; rewrite IH//lvlF_incr//. Qed.
+
+    Lemma all2_lvlF_incr {ca}:
+      all (all lvlD) ca -> incr_cuts ca = ca.
+    Proof. elim: ca => //x xs IH/=/andP[] H1 H2. rewrite IH//all_lvlF_incr//. Qed.
+
+    Lemma lvlF_incrT {x}: lvlD (incr_cut x).
+    Proof. case: x => //-[]//. Qed.
+
+    Lemma all_lvlF_incrT {ca}:
+      all lvlD (map incr_cut ca).
+    Proof. elim: ca => // x xs/=->; rewrite lvlF_incrT//. Qed.
+
+    Lemma all2_lvlF_incrT {ca}:
+      all (all lvlD) (incr_cuts ca).
+    Proof. elim: ca => // x xs/=->; rewrite all_lvlF_incrT//. Qed.
+
+    Lemma lvlF_base_and_ko_s2l {B l}:
+      base_and_ko B -> all (all lvlD) l -> all (all lvlD) (state_to_list B l).
+    Proof. elim: B l => //=-[]//. Qed.
+
+    Lemma lvlF_base_or_ko_s2l {B l}:
+      base_or_aux_ko B -> all (all lvlD) l -> all (all lvlD) (state_to_list B l).
+    Proof. 
+      elim: B l => //[|[]]//.
+      move=> A HA s B HB l/=/andP[bA bB] H.
+      rewrite all2_lvlF_incrT//.
+    Qed.
+
+    Lemma lvlF_add_ca {b ca x}: lvlD ca -> lvlD (add_ca b x ca).
+    Proof. case: ca => //= -[]// l _; rewrite orbT//. Qed.
+
+    Lemma all_lvlF_add_ca {ca b x}: (all lvlD) ca -> (all lvlD) ((map (add_ca b x)) ca).
+    Proof. elim: ca b x => //x xs IH b y/= /andP[H1 H2]; rewrite IH//lvlF_add_ca//. Qed.
+
+    Lemma all2_lvlF_add_ca {ca b x}: all (all lvlD) ca -> all (all lvlD) (map (map (add_ca b x)) ca).
+    Proof. elim: ca x => //x xs IH y/=/andP[H1 H2]; rewrite IH//all_lvlF_add_ca//. Qed.
+
+  End lvlD.
+
+  Section is_nil.
+    Definition is_nil {T : Type} (l: list T) := match l with [::] => true | _ => false end.
+
+    Lemma is_nil_incr_cuts {r}:
+      is_nil (map incr_cut r) = is_nil r.
+    Proof. elim: r => //A HA IH /=/andP[] H /IH->. Qed.
+
+    Lemma all_is_nil_incr_cuts {r}:
+      all is_nil (incr_cuts r) = all is_nil r.
+    Proof. elim: r=>//x xs /=->; rewrite is_nil_incr_cuts//. Qed.
+
+    Lemma is_nil_add_ca {ca b r}:
+      is_nil (map (add_ca b ca) r) = is_nil r.
+    Proof. elim: r=>//x xs /=->//. Qed.
+
+    Lemma all_is_nil_add_ca {ca b r}:
+      all is_nil (map (map (add_ca b ca)) r) = all is_nil r.
+    Proof. elim: r=>//x xs /=->; rewrite is_nil_add_ca//. Qed.
+
+    Lemma all_is_nil_make_lb0 {rs l}:
+      all is_nil rs -> all is_nil (make_lB0 rs l).
+    Proof.
+      rewrite/make_lB0.
+      elim: rs l => //-[]//= xs IH l H.
+      rewrite all_cat IH// map_id.
+    Abort.
+  End is_nil.
+
+  Section size.
+    Lemma size_o_map {T R: Type} (F:T->R) L: (size \o map F) L = size L.
+    Proof. elim: L => //= _ l->//. Qed.
+
+    Lemma size_o_cat {T: Type} L (x y: list T): 
+      size x = size y -> (size \o [eta cat x]) L = (size \o [eta cat y]) L.
+    Proof. case: L x y => [|w ws] x y /=; rewrite ?cats0//!size_cat => ->//. Qed.  
+    
+    Lemma size_o_map_map {T R: Type} {F:T->R} L: map (size \o map F) L = map size L.
+    Proof. elim: L => //= x xs->/=; f_equal; rewrite -(size_o_map F x)//. Qed.
+
+    Lemma size_o_cat_map {T: Type} L (x: list T): 
+      map (size \o [eta cat x]) L = map (fun y => size x + size y) L. 
+    Proof. elim: L => //y ys/=->; rewrite size_cat //. Qed.
+
+    Lemma size_prep {T: Type} {y: list T} {L1 L2:list (list T)}:
+      [seq size y0 | y0 <- L1] = [seq size y0 | y0 <- L2] ->
+        [seq size y + size y0 | y0 <- L1] = [seq size y + size y0 | y0 <- L2].
+    Proof. move=> H. rewrite map_comp H !(map_comp _ _ L2)//. Qed.
+
+    Lemma size_flatten {T:Type} {L1 L2 xs ys: list (list T)}:
+      [seq size ii | ii <- xs] = [seq size ii | ii <- ys] ->
+      [seq size ii | ii <- L1] = [seq size ii | ii <- L2] ->
+        [seq size ii | ii <- [seq la ++ lb | la <- xs, lb <- L1]] =
+          [seq size ii | ii <- [seq la ++ lb | la <- ys, lb <- L2]].
+    Proof.
+      elim: xs ys L1 L2=> [|x xs IH] [|y ys]//=L1 L2.
+      move=>[] H1 H2 H3.
+      have:= IH _ _ _ H2 H3.
+      rewrite 2!map_cat=>->; f_equal.
+      rewrite -2!map_comp 2!size_o_cat_map map_comp H1 H3 3!(map_comp _ _ L2)//.
+    Qed.
+  End size.
 
   Section state_to_list_prop.
-
-   (* Definition add_ca' (l2 : list alt) gl : G :=
-    match gl with
-    | call _ _ => gl
-    | cut l1 => cut (if length l1 == 0 then l1 else l1 ++ l2) 
-    end.
-
-    Lemma state_to_list_state_bt_app {A xs ys r}:
-      xs <> [::] ->
-        state_to_list A (xs ++ ys) = r ->
-          r = map (map (add_ca' ys)) (state_to_list A xs).
-    Proof. (This is false)
-    Abort. *)
 
     Lemma state_to_list_dead {A l}: is_dead A -> state_to_list A l = [::].
     Proof.
@@ -540,35 +668,6 @@ Module Nur (U : Unif).
       - move=> /= A HA s B HB l /andP[bA bB]; rewrite HB//=base_and_ko_state_to_list//.
       - move=>[]//.
     Qed.
-
-    (* Lemma success_state_to_list {A} m:
-      success A -> exists r, state_to_list A m = [::] :: r.
-    Proof.
-      elim: A m => //.
-      - by eexists.
-      - move=> A HA s B HB m/=.
-        case: ifP => [dA sB|dA sA].
-          have [r H]:= HB m sB.
-          eexists; rewrite H (state_to_list_dead dA)//.
-        have [r H]:= HA (state_to_list B m ++ m) sA; eexists.
-        rewrite H//.
-      - move=> A HA B0 HB0 B HB m /=/andP[sA sB].
-        have [r1 H1] := HA m sA.
-        have [r2 H2] := HB m sB.
-        rewrite H1 H2/=map_id.
-        case: r2 H2 => /=[|x xs].
-          by eexists.
-        by eexists.
-    Qed. *)
-
-    (* Lemma propagate_cut_clean_success {A}: propagate_cut (clean_success A) = propagate_cut A.
-    Proof. 
-      elim: A => //.
-      - move=> A HA s B HB/=; rewrite fun_if if_same//.
-      - move=> A HA B0 _ B HB/=; rewrite (fun_if propagate_cut)/=.
-        rewrite HB if_same//.
-    Qed. *)
-
 
     Lemma success_state_to_list {A m}:
       success A ->
@@ -596,49 +695,6 @@ Module Nur (U : Unif).
       by move=>[].
     Qed.
 
-    Lemma success_next_alt_state_to_list {s1 A}:
-      valid_state A -> success A -> next_alt s1 A = None -> 
-        forall l, exists x, state_to_list A l = [::x].
-    Proof.
-      elim: A s1 => //.
-      - by exists [::].
-      - move=> A HA s B HB s1/=.
-        case: ifP => [dA vB sB|dA /andP[vA bB] sA] + l.
-          rewrite state_to_list_dead//=.
-          case X: next_alt => [[]|]//.
-          have [x ->]:= HB _ vB sB X l.
-          by eexists.
-        case X: next_alt => [[]|]//.
-        have H:= bbOr_valid bB.
-        case: ifP => dB.
-          rewrite valid_state_dead// in H.
-        (* case: ifP => // fB. *)
-        case Y: next_alt => [[]|]// _.
-        have [x H1] := HA _ vA sA X (state_to_list B l ++ l).
-        rewrite H1/=.
-        have:= bB; rewrite /bbOr.
-        case Z: base_or_aux => //=.
-          have H2 := next_alt_aux_base_or_none Z Y.
-          by subst.
-        move=> bB0'.
-        rewrite (base_or_aux_ko_state_to_list bB0')/=.
-        by eexists.
-      - move=> A HA B0 _ B HB s1 /=/and5P[oA vA aB].
-        case: ifP => //sA vB/=bB0 sB + l.
-        rewrite success_is_dead// success_failed//.
-        case X: next_alt => [[]|]//.
-        have [x H1] := HB _ vB sB X l; rewrite H1.
-        case Y: next_alt => [[s2 C]|]//.
-          move: bB0; rewrite /bbAnd.
-          case Z: base_and => //=.
-            rewrite base_and_failed//.
-          move=> bB0; rewrite (base_and_ko_failed bB0) // (base_and_ko_state_to_list bB0)//=.
-          rewrite success_state_to_list//add_alt_empty1 make_lB0_empty2 cats0.
-          rewrite make_lB_empty2; by eexists.
-        have [y H2] := HA _ vA sA Y l.
-        rewrite H2/= add_alt_empty2/=; by eexists.
-    Qed.
-
     Lemma bbOr_next_alt_none {s B l}:
       bbOr B -> next_alt s B = None -> state_to_list B l = [::].
     Proof.
@@ -654,20 +710,56 @@ Module Nur (U : Unif).
         rewrite next_alt_aux_base_and//.
     Qed.
 
-    Lemma base_or_aux_next_alt_some {s B s1 D l}:
-      base_or_aux B -> next_alt s B = Some (s1, D) -> state_to_list B l = state_to_list D l.
+    Lemma bbOr_next_alt_some {s1 s2 B C l}:
+      bbOr B -> next_alt s1 B = Some(s2, C) -> state_to_list B l = state_to_list C l.
     Proof.
-      elim: B s s1 D l => //.
-      - move=>/=???? _[_<-]//.
-      - move=> A HA s B HB s1 s3 C l/=/andP[bA bB].
-        rewrite base_and_dead//next_alt_aux_base_and//.
-        move=>[_<-]//.
-      - move=> []// p a _ B0 _ B HB s1 s2 C l/=/andP[/eqP->bB].
+      elim: B s1 s2 C l => //.
+      - move=> /= ?????[_<-]//.
+      - move=> A HA s B HB s1 s2 C l/=; rewrite /bbOr/=.
+        move=>/orP[]/andP[bA bB].
+          rewrite base_and_dead// next_alt_aux_base_and//.
+          move=>[_<-]//.
+        rewrite base_and_ko_is_dead// base_or_aux_is_dead//.
+        rewrite(next_alt_aux_base_or_ko bB) (next_alt_aux_base_and_ko bA)//.
+      - move=> []//p a _ B0 _ B HB s1 s2 C l/=; rewrite/bbOr/=orbF => /andP[/eqP->bB].
         rewrite next_alt_aux_base_and// => -[_<-]//.
     Qed.
 
+    Lemma success_next_alt_state_to_list {s1 A l}:
+      valid_state A -> success A -> next_alt s1 A = None -> 
+        state_to_list A l = [::[::]].
+    Proof.
+      elim: A s1 l => //.
+      - move=> A HA s B HB s1 l/=.
+        case: ifP => [dA vB sB|dA /andP[vA bB] sA].
+          rewrite state_to_list_dead//=.
+          case X: next_alt => [[]|]//.
+          rewrite (HB _ _ vB sB X)//.
+        case X: next_alt => [[]|]//.
+        have H:= bbOr_valid bB.
+        case: ifP => dB.
+          rewrite valid_state_dead// in H.
+        (* case: ifP => // fB. *)
+        case Y: next_alt => [[]|]// _.
+        have H1 := HA _  (state_to_list B l ++ l) vA sA X.
+        rewrite H1 (bbOr_next_alt_none bB Y)//.
+      - move=> A HA B0 _ B HB s1 l /=/and5P[oA vA aB].
+        case: ifP => //sA vB/=bB0 sB.
+        rewrite success_is_dead// success_failed//.
+        case X: next_alt => [[]|]//.
+        have H1 := HB _ _ vB sB X; rewrite H1.
+        case Y: next_alt => [[s2 C]|]//.
+          move: bB0; rewrite /bbAnd.
+          case Z: base_and => //=.
+            rewrite base_and_failed//.
+          move=> bB0; rewrite (base_and_ko_failed bB0) // (base_and_ko_state_to_list bB0)//=.
+          rewrite success_state_to_list//add_alt_empty1 make_lB0_empty2 cats0.
+          rewrite make_lB_empty2; by eexists.
+        have H2 := HA _ l vA sA Y.
+        rewrite H2 add_alt_empty2//.
+    Qed.
 
-    Lemma failed_next_alt_state_to_list {s1 A}:
+    Lemma failed_next_alt_none_state_to_list {s1 A}:
       valid_state A -> failed A -> next_alt s1 A = None -> 
         forall l, state_to_list A l = [::].
     Proof.
@@ -700,8 +792,8 @@ Module Nur (U : Unif).
             case: state_to_list => //*.
             rewrite add_alt_empty4 make_lB0_empty2//.
           move=> _ l.
-          have [x H]:= success_next_alt_state_to_list vA sA Y l.
-          rewrite H add_alt_empty2 (HB s1)//.
+          rewrite (success_next_alt_state_to_list vA sA Y) add_alt_empty2/=.
+          rewrite map_id (HB s1)//.
         case: ifP => //fA bB _ + l.
         case: ifP => //dA.
           rewrite (state_to_list_dead dA)//.
@@ -718,38 +810,172 @@ Module Nur (U : Unif).
         have -> //:= HA _ vA fA X l.
     Qed.
 
-    Lemma size_o_map {T R: Type} (F:T->R) L: (size \o map F) L = size L.
-    Proof. elim: L => //= _ l->//. Qed.
-
-    Lemma size_o_cat {T: Type} L (x y: list T): 
-      size x = size y -> (size \o [eta cat x]) L = (size \o [eta cat y]) L.
-    Proof. case: L x y => [|w ws] x y /=; rewrite ?cats0//!size_cat => ->//. Qed.  
-    
-    Lemma size_o_map_map {T R: Type} {F:T->R} L: map (size \o map F) L = map size L.
-    Proof. elim: L => //= x xs->/=; f_equal; rewrite -(size_o_map F x)//. Qed.
-
-    Lemma size_o_cat_map {T: Type} L (x: list T): 
-      map (size \o [eta cat x]) L = map (fun y => size x + size y) L. 
-    Proof. elim: L => //y ys/=->; rewrite size_cat //. Qed.
-
-    Lemma size_prep {T: Type} {y: list T} {L1 L2:list (list T)}:
-      [seq size y0 | y0 <- L1] = [seq size y0 | y0 <- L2] ->
-        [seq size y + size y0 | y0 <- L1] = [seq size y + size y0 | y0 <- L2].
-    Proof. move=> H. rewrite map_comp H !(map_comp _ _ L2)//. Qed.
-
-    Lemma size_flatten {T:Type} {L1 L2 xs ys: list (list T)}:
-      [seq size ii | ii <- xs] = [seq size ii | ii <- ys] ->
-      [seq size ii | ii <- L1] = [seq size ii | ii <- L2] ->
-        [seq size ii | ii <- [seq la ++ lb | la <- xs, lb <- L1]] =
-          [seq size ii | ii <- [seq la ++ lb | la <- ys, lb <- L2]].
+    Lemma base_or_aux_next_alt_some {s B s1 D l}:
+      base_or_aux B -> next_alt s B = Some (s1, D) -> state_to_list B l = state_to_list D l.
     Proof.
-      elim: xs ys L1 L2=> [|x xs IH] [|y ys]//=L1 L2.
-      move=>[] H1 H2 H3.
-      have:= IH _ _ _ H2 H3.
-      rewrite 2!map_cat=>->; f_equal.
-      rewrite -2!map_comp 2!size_o_cat_map map_comp H1 H3 3!(map_comp _ _ L2)//.
+      elim: B s s1 D l => //.
+      - move=>/=???? _[_<-]//.
+      - move=> A HA s B HB s1 s3 C l/=/andP[bA bB].
+        rewrite base_and_dead//next_alt_aux_base_and//.
+        move=>[_<-]//.
+      - move=> []// p a _ B0 _ B HB s1 s2 C l/=/andP[/eqP->bB].
+        rewrite next_alt_aux_base_and// => -[_<-]//.
     Qed.
 
+
+    Lemma clean_successP {s1 s2 A B l}:
+      valid_state A -> success A ->
+        next_alt s1 A = Some (s2, B) -> state_to_list B l = state_to_list (clean_success A) l.
+    Proof.
+      elim: A s1 s2 B l => //.
+      - move=> A HA s B HB s2 s3 C l/=.
+        case: ifP => //[dA vB sB|dA /andP[vA bB] sA].
+          case Y: next_alt => [[s6 E]|]//[_<-]/=.
+          rewrite !(state_to_list_dead dA)/=.
+          f_equal; apply: HB vB sB Y.
+        case nA: next_alt => [[s6 E]|].
+          move=>[_<-]/=; f_equal.
+          have ->// := HA _ _ _ _ vA sA nA.
+        case : ifP => //dB.
+        case nB: next_alt => //[[s6 E]][_<-]/=.
+        rewrite (state_to_list_dead is_dead_dead)/=.
+        have H := success_next_alt_state_to_list vA sA nA.
+        have ->/= := state_to_list_empty_clean sA (H _).
+        move: bB; rewrite /bbOr => /orP[] bB.
+          have ->// := base_or_aux_next_alt_some bB nB.
+        by rewrite (next_alt_aux_base_or_ko bB) in nB.
+      - move=> A HA B0 _ B HB s2 s3 C l/=/and5P[oA vA eB] + + /andP[sA sB].
+        rewrite sA/==>vB bB0.
+        rewrite success_is_dead//success_failed//.
+        case nB: next_alt => [[s7 E]|].
+          move=>[_<-]/=.
+          rewrite !(success_state_to_list sA)!add_alt_empty1.
+          have {}HB := (HB _ _ _ _ vB sB nB).
+          rewrite HB//.
+        case nA': next_alt => [[s7 F]|]//.
+        case: ifP => // fB0[_<-]/=.
+        move: bB0; rewrite /bbAnd => /orP[bB|]; last first.
+          move=>/base_and_ko_failed; rewrite fB0//.
+        have [x Hb]:= base_and_state_to_list bB.
+        have lvlS := base_and_lvlt bB (Hb [::]).
+        have ->/= := HA _ _ _ _ vA sA nA'.
+        have H := success_next_alt_state_to_list vB sB nB.
+        rewrite (state_to_list_empty_clean sB (H _)).
+        rewrite (success_state_to_list sA)/=add_alt_empty1.
+        case X: (state_to_list (clean_success A)) => [|b bs]//.
+        rewrite /add_alt/make_lB/make_lB0/= !Hb/=.
+        rewrite (all_lvlt_add_caF lvlS)//.
+    Qed.
+
+
+    Lemma failed_next_alt_some_state_to_list {s1 A s2 B l}:
+      valid_state A -> failed A -> next_alt s1 A = Some(s2, B) -> 
+        state_to_list A l = state_to_list B l.
+    Proof.
+      elim: A s1 s2 B l => //.
+      - move=> A HA s B HB s1 s2 C l/=.
+        case: ifP => [dA vB fB|dA /andP[vA bB] fA].
+          case X: next_alt => [[s3 D]|]//[_<-]/=.
+          rewrite !(state_to_list_dead dA)//=(HB _ _ _ _ vB fB X)//.
+        case X: next_alt => [[s3 D]|]//.
+          move=>[_<-]/=.
+          rewrite (HA _ _ _ _ vA fA X)//.
+        case: ifP => dB//.
+        case Y: next_alt => [[s3 D]|]//[_<-]/=.
+        rewrite (state_to_list_dead is_dead_dead)/=.
+        rewrite (failed_next_alt_none_state_to_list vA fA X)/=.
+        rewrite (bbOr_next_alt_some bB Y)//.
+      - move=> A HA B0 HB0 B HB s1 s2 C l /=/and5P[oA vA aB].
+        case: (ifP (is_dead _)) => //dA.
+        case: ifP => /=[sA vB bB0|sA/eqP->].
+          rewrite success_failed//= => fB.
+          case X: next_alt => [[s3 D]|]//.
+            move=>[_<-]/=.
+            rewrite (HB _ _ _ _ vB fB X)//.
+          case Y: next_alt => [[s3 D]|]//.
+          case: ifP => fB0//[_<-]/=.
+          rewrite (clean_successP vA sA Y).
+          move: bB0; rewrite /bbAnd => /orP[]bB; last first.
+            by rewrite (base_and_ko_failed bB) in fB0.
+          have [hd H]:= base_and_state_to_list bB.
+          rewrite H.
+          rewrite (failed_next_alt_none_state_to_list vB fB X).
+          rewrite success_state_to_list //add_alt_empty1 make_lB_empty1/=.
+          case sCA: (state_to_list (clean_success _))=>//[z zs].
+          rewrite /add_alt/make_lB/make_lB0/=.
+          have lhd := base_and_lvlt bB (H [::]).
+          rewrite all_lvlt_add_caF//.
+        case: ifP => //fA bB _.
+        case X: next_alt => [[s3 D]|]//.
+        case:ifP => fB => //-[_<-]/=.
+        rewrite (HA _ _ _ _ vA fA X)//.
+    Qed.
+
+    Lemma next_alt_none_s2l {s B} l:
+      valid_state B -> next_alt s B = None -> exists r, state_to_list B l = r /\ all is_nil r.
+    Proof.
+      elim: B s l => //; try by eexists.
+      - move=> A HA s B HB s1 l/=.
+        case:ifP => [dA vB|dA /andP[vA bB]].
+          rewrite state_to_list_dead//=.
+          case nB: next_alt => [[]|]//.
+          have [r [H1 H2]]:= HB _ l vB nB.
+          rewrite H1; eexists; split => //.
+          by rewrite all_is_nil_incr_cuts.
+        case nA: next_alt => [[]|]//.
+        have [r [H H1]]:= HA _ (state_to_list B l ++ l) vA nA.
+        rewrite H.
+        case:ifP => //dB.
+          rewrite state_to_list_dead//cats0.
+          eexists; split => //.
+          rewrite all_is_nil_incr_cuts. rewrite all_is_nil_add_ca//.
+        case nB: next_alt => [[z zs]|]//.
+        have [r1 [H2 H3]]:= HB _ l (bbOr_valid bB) nB.
+        rewrite H2; eexists; split => //.
+        rewrite all_is_nil_incr_cuts all_cat H3 all_is_nil_add_ca H1//.
+      - move=> A HA B0 _ B HB s l /=.
+        case:(ifP (is_dead _)) => //dA.
+          rewrite state_to_list_dead//; by eexists.
+        case: (ifP (failed _)) => fA//.
+          rewrite failed_success//= => /and5P[oA vA aB /eqP-> bB].
+          case nA: next_alt => [[x xs]|]//.
+            case:ifP => //fB0.
+            move: bB; rewrite/bbAnd=>/orP[].
+              by move=>/base_and_failed; rewrite fB0.
+            move=>/base_and_ko_state_to_list->.
+            case: state_to_list => //; eexists; split => //.
+            rewrite add_alt_empty3//.
+          have [r [H H1]]:= HA _ l vA nA.
+          rewrite (failed_next_alt_none_state_to_list vA fA nA).
+          eexists; split => //.
+        move=>/and5P[oA vA aB].
+        case nB: next_alt => [[x xs]|]//.
+        case:ifP => //=[sA vB bB0|sA/eqP->/[dup]/base_and_valid vB bB]; 
+        have [r [H1 H2]]:= HB _ l vB nB; rewrite H1.
+          case nA: next_alt => [[x xs]|]//.
+            case:ifP => //fB0.
+            move:bB0; rewrite/bbAnd=>/orP[].
+              move=>/base_and_failed; rewrite fB0//.
+            move=>/base_and_ko_state_to_list->.
+            rewrite success_state_to_list// add_alt_empty1 make_lB0_empty2 make_lB_empty2 cats0.
+            eexists; split => //.
+          have [r1 []]:= HA _ l vA nA.
+          rewrite (success_next_alt_state_to_list vA sA nA).
+          move=> ?; subst; eexists; split; auto.
+          rewrite add_alt_empty2 map_id//.
+        case nA: next_alt => [[x xs]|]//.
+          rewrite base_and_failed//.
+        have [[|r1 r1s] [->]]:= HA _ l vA nA.
+          eexists; auto.
+        case: r1 => //=n _.
+        rewrite add_alt_empty1.
+        eexists; split=>//.
+        rewrite all_cat/make_lB/make_lB0.
+        rewrite all_is_nil_add_ca H2/=.
+        move: H2 n; clear.
+        elim: r1s r => //=-[]// xs IH r H1/andP[H2 H3].
+        rewrite all_cat map_id H1 IH//.
+    Qed.
 
     Lemma state_to_list_same_shape {r1 r2 A l1 l2}: 
       state_to_list A l1 = r1 -> state_to_list A l2 = r2 -> shape r1 = shape r2.
@@ -785,10 +1011,6 @@ Module Nur (U : Unif).
 
     Lemma state_to_list_empty {A l1 l2}: state_to_list A l1 = [::] -> state_to_list A l2 = [::].
     Proof. move=>/state_to_list_same_shape => /(_ _ l2 erefl); case: state_to_list => //. Qed.
-
-    Lemma state_to_list_cons_bt {A l1 l2 x xs}: state_to_list A l1 = x :: xs -> exists y ys, state_to_list A l2 = y::ys.
-    Proof. move=>/state_to_list_same_shape => /(_ _ l2 erefl); case: state_to_list => //; by do 2 eexists. Qed.
-
 
   End state_to_list_prop.
 
@@ -849,39 +1071,6 @@ Module Nur (U : Unif).
         have [y[ys->]]:= HB (base_and_valid bB) fB l.
         by do 2 eexists.
     Qed.
-
-    (* Definition lvl0 A:= match A with cut n _ => nat_eqb n 0 | _ => true end. *)
-    Definition lvl0 A:= match A with cut b1 _ => b1 | _ => true end.
-
-    Lemma base_and_state_to_list {A}: base_and A -> exists hd, forall l, state_to_list A l = [::hd].
-    Proof.
-      elim: A => //.
-      - by eexists.
-      - move=> []//p a _ B0 _ B HB/=/andP[/eqP->bB].
-        have [hd H]/= := HB bB.
-        case: a => [|t]; eexists => l; rewrite H //.
-    Qed.
-
-    Lemma base_and_lvl0 {A l hd}: 
-      base_and A -> state_to_list A l = [::hd] -> all lvl0 hd.
-    Proof.
-      elim: A l hd => //.
-      - move=> l hd _ [<-]//.
-      - move=> []// p a _ B0 _ B HB l hd/=/andP[/eqP->bB].
-        have [hd1 H]:= base_and_state_to_list bB; rewrite H.
-        case: a => //[|t]; rewrite add_alt_empty2/==>-[?]; subst => /=; apply: HB bB (H [::]).
-    Qed.
-
-  Lemma lvl0_add_ca0 {y l}:
-    lvl0 y -> add_ca0 l y = y.
-  Proof. case: y => //-[]//. Qed.
-
-  Lemma all_lvl0_add_ca0 {y l}:
-    all lvl0 y -> [seq add_ca0 l e | e <- y] = y.
-  Proof.
-    elim: y l => //=x xs IH l/andP[lx lxs].
-    rewrite IH//lvl0_add_ca0//.
-  Qed.
 
 
     Lemma next_alt_state_to_list_old {s1 A s2 B}:
@@ -1005,7 +1194,7 @@ Module Nur (U : Unif).
           move=> /=[?]; subst => /cats20[]; subst; case: ws H2 => //= H3 _; rewrite (HB _ _ _ sB vB H3).
             case: ys H1 => // SA.
             rewrite (HA _ _ _ sA vA SA)//.
-        move=>/[dup]H/base_and_ko_state_to_list->/=; rewrite flatten_empty add_ca0_empty map_add0_cas_empty cats0.
+        move=>/[dup]H/base_and_ko_state_to_list->/=; rewrite flatten_empty add_ca_empty map_add0_cas_empty cats0.
         case: ws H2 => // SB/=[?]; subst.
         rewrite (HB _ _ _ sB vB SB).
         rewrite (base_and_ko_failed H)//; case: next_alt => [[]|]//.
@@ -1100,8 +1289,7 @@ Module Nur (U : Unif).
           rewrite base_and_ko_failed//.
           rewrite (base_and_ko_state_to_list bB)//.
           case: state_to_list => //=*; rewrite add_alt_empty3//.
-        have /=[x H]:= success_next_alt_state_to_list (valid_state_expand vA eA) sA' nA' l.
-        rewrite (expand_solved_same eA) H add_alt_empty2//.
+        rewrite (expand_solved_same eA) (success_next_alt_state_to_list (valid_state_expand vA eA) sA' nA')//.
     Qed.
 
     Lemma next_alt_propagate_cut {s1 s2 A B}:
@@ -1128,48 +1316,29 @@ Module Nur (U : Unif).
         case: ifP => //fB0[_<-]//.
     Qed.
 
-    Lemma clean_successP {s1 s2 A B l}:
-      valid_state A -> success A ->
-        next_alt s1 A = Some (s2, B) -> state_to_list B l = state_to_list (clean_success A) l.
+  
+    Lemma expand_failure_state_to_list_same {s A B l}:
+      (* valid_state A ->  *)
+        expand s A = Failure B ->
+            state_to_list A l = state_to_list B l.
     Proof.
-      elim: A s1 s2 B l => //.
-      - move=> A HA s B HB s2 s3 C l/=.
-        case: ifP => //[dA vB sB|dA /andP[vA bB] sA].
-          case Y: next_alt => [[s6 E]|]//[_<-]/=.
-          rewrite !(state_to_list_dead dA)/=.
-          f_equal; apply: HB vB sB Y.
-        case nA: next_alt => [[s6 E]|].
-          move=>[_<-]/=; f_equal.
-          have ->// := HA _ _ _ _ vA sA nA.
-        case : ifP => //dB.
-        case nB: next_alt => //[[s6 E]][_<-]/=.
-        rewrite (state_to_list_dead is_dead_dead)/=.
-        have /= [x H] := (success_next_alt_state_to_list vA sA nA) (state_to_list B l ++ l).
-        have ->/= := state_to_list_empty_clean sA H.
-        move: bB; rewrite /bbOr => /orP[] bB.
-          have ->// := base_or_aux_next_alt_some bB nB.
-        by rewrite (next_alt_aux_base_or_ko bB) in nB.
-      - move=> A HA B0 _ B HB s2 s3 C l/=/and5P[oA vA eB] + + /andP[sA sB].
-        rewrite sA/==>vB bB0.
-        rewrite success_is_dead//success_failed//.
-        case nB: next_alt => [[s7 E]|].
-          move=>[_<-]/=.
-          rewrite !(success_state_to_list sA)!add_alt_empty1.
-          have {}HB := (HB _ _ _ _ vB sB nB).
-          rewrite HB//.
-        case nA': next_alt => [[s7 F]|]//.
-        case: ifP => // fB0[_<-]/=.
-        move: bB0; rewrite /bbAnd => /orP[bB|]; last first.
-          move=>/base_and_ko_failed; rewrite fB0//.
-        have [x Hb]:= base_and_state_to_list bB.
-        have lvl0 := base_and_lvl0 bB (Hb [::]).
-        have ->/= := HA _ _ _ _ vA sA nA'.
-        have /= [y H]:= success_next_alt_state_to_list vB sB nB l.
-        rewrite (state_to_list_empty_clean sB H).
-        rewrite (success_state_to_list sA)/=add_alt_empty1.
-        case X: (state_to_list (clean_success A)) => [|b bs]//.
-        rewrite /add_alt/make_lB/make_lB0/= !Hb/=.
-        rewrite (all_lvl0_add_ca0 lvl0)//.
+      elim: A s B l => //.
+      - move=> /= ??? [<-]//.
+      - move=> /= ??? [<-]//.
+      - move=> p [|t]//.
+      - move=> A HA s B HB /= s1 C l.
+        case: ifP => dA.
+          case eB: expand => // [B'] [<-]/=.
+          rewrite 2!(state_to_list_dead dA)//=.
+          f_equal; apply: HB eB.
+        case eA: expand => //[A'][<-]/=.
+        have ->// := HA _ _ _ eA.
+      - move=> A HA B0 _ B HB s C l/=.
+        case eA: expand => //[A'|s1 A'].
+          move=>[<-]; rewrite (HA _ _ _ eA)//.
+        have [??] := (expand_solved_same eA); subst.
+        case eB: expand => //[B'][<-]/=.
+        rewrite (HB _ _ _ eB)//.
     Qed.
   
     Lemma expand_failure_next_alt_state_to_list_cons {s A B s1 s2 C l}:
@@ -1237,8 +1406,8 @@ Module Nur (U : Unif).
         have H2 := clean_successP vA sA nA'.
         rewrite /add_alt/make_lB/make_lB0/=H1 H2.
         case SA: state_to_list => //=.
-        have lvl0:= base_and_lvl0 bB0 (H1 [::]).
-        rewrite (all_lvl0_add_ca0 lvl0)//.
+        have lvlS:= base_and_lvlt bB0 (H1 [::]).
+        rewrite (all_lvlt_add_caF lvlS)//.
     Qed.
 
     Lemma expandedb_failure_next_alt_state_to_list_cons {s1 s2 A B C b1}:
@@ -1279,28 +1448,17 @@ Module Nur (U : Unif).
   End list_cons.
 
 
-  Lemma expand_done {s A s1 B} l:
+  Lemma expand_solved {s A s1 B} l:
     expand s A = Solved s1 B ->
     exists x xs,
       state_to_list A l = x :: xs /\
       nur s x xs s1 (state_to_list (clean_success B) l).
   Proof.
-    move=> H.
-    have H1 := (expand_solved_same H).
-    rewrite 2!H1 in H.
-    rewrite 2!H1.
+    move=>/[dup] /expand_solved_same [->->] H.
     do 2 eexists; split.
       apply: success_state_to_list (expand_solved_success H).2.
     apply: StopE.
   Qed.
-
-  Fixpoint get_ca (A: state) bt :=
-    match A with
-    | Goal _ Cut => bt
-    | Goal _ _ | OK | Dead | Bot | Top => bt
-    | And A _ B => if success A then get_ca B bt else get_ca A bt
-    | Or A s B => if is_dead A then get_ca B bt else get_ca A (Or bt s B)
-    end.
 
   Lemma state_to_list_cutr_empty {A l}:
     valid_state A -> state_to_list (cutr A) l = [::].
@@ -1338,21 +1496,15 @@ Module Nur (U : Unif).
       rewrite HA//add_alt_empty2/=map_id HB//.
   Qed.
 
-  Definition is_cut A:= match A with Goal _ Cut => true | _ => false end.
-
   Lemma expand_cb_state_to_list1 {s1 A s2 B} l1:
     valid_state A -> expand s1 A = CutBrothers s2 B -> 
       exists x tl, 
-        ((forall l, (state_to_list A l1 = [:: [::cut true [::] & x] & tl]) * (state_to_list B l = [::x])) * (all lvl0 x))%type.
+        ((forall l, (state_to_list A l1 = [:: [::cut false [::] & x] & tl]) * (state_to_list B l = [::x])) * (all lvlS x))%type.
   Proof.
     elim: A s1 s2 B l1 => //.
     - move=> p []//= ?????[_<-]/=; by do 2 eexists.
     - move=> A HA s B HB s1 s2 C l1 /=.
       case: ifP => [dA vB|dA/andP[vA bB]]; case eB: expand => //[s1' B'][??]; subst.
-      (* move=>/=.
-      have [x[tl H]] := HB _ _ _ l1 vB eB.
-      do 2 eexists; move=> l.
-      rewrite 2!(state_to_list_dead dA)/=2!H//. *)
     - move=> A HA B0 _ B HB s1 s2 C l1/=/and5P[oA vA aB].
       case eA: expand => //[s3 A'|s3 A'].
         rewrite (expand_not_solved_not_success eA erefl)/=(expand_not_failed eA notF).
@@ -1365,9 +1517,9 @@ Module Nur (U : Unif).
           split => //.
           rewrite/add_alt/make_lB/make_lB0/=.
           repeat f_equal.
-          have:= base_and_lvl0 bB (H1 [::]).
-          move=>/all_lvl0_add_ca0->//.
-        rewrite all_cat H4// (base_and_lvl0 bB (H1 [::]))//.
+          have:= base_and_lvlt bB (H1 [::]).
+          move=>/all_lvlt_add_caF ->//.
+        rewrite all_cat H4// (base_and_lvlt bB (H1 [::]))//.
       have [sA sA'] := expand_solved_success eA.
       rewrite sA/==> vB bB0.
       case eB: expand => //[s4 B'] [_<-]/=.
@@ -1378,493 +1530,347 @@ Module Nur (U : Unif).
       do 2 eexists; split.
         move=> l; rewrite 2!(H l).
         rewrite state_to_list_cutl//add_alt_empty2//=; repeat split => //.
-          rewrite all_lvl0_add_ca0//H//.
-        rewrite all_lvl0_add_ca0//H//.
+          rewrite all_lvlt_add_caF//H//.
+        rewrite all_lvlt_add_caF//H//.
   Qed.
 
-  Lemma boh {s1 A s2 B bt1 bt2 z zs}:
-      valid_state A ->
-        expandedb s1 A (Done s2 B) false ->
-          state_to_list A bt1 = z :: zs ->
-            map (add_ca bt2) z = z.
-  Proof. (* è falso *)
-  Abort.
-
-  (* this is the shape a state A should have if expandedb s1 A (Done s2 B) b *)
-  Fixpoint exp_done_shape A :=
-    match A with
-    | OK | Top | Goal _ Cut => true
-    | And A _ B => exp_done_shape A && exp_done_shape B
-    | Or A _ B => if is_dead A then exp_done_shape B else exp_done_shape A
-    | _ => false
-    end.
+  Section exp_done_rel.
+    (* this is the shape a state A should have if expandedb s1 A (Done s2 B) b *)
+    Fixpoint exp_done_shape A :=
+      match A with
+      | OK | Top | Goal _ Cut => true
+      | And A _ B => exp_done_shape A && exp_done_shape B
+      | Or A _ B => if is_dead A then exp_done_shape B else exp_done_shape A
+      | _ => false
+      end.
 
     Inductive has_cut := sup | no | deep.
     derive has_cut.
     HB.instance Definition _ := hasDecEq.Build has_cut has_cut_eqb_OK.
 
-  (*  
-    given two states A and B such that (exp_done_shape A),
-    returns (b * deep_cut * has_cut) where
-    - b tells if B is a valid evolution of A after a call to expand
-    - deep_cut tells a deep cut has been executed
-    - has_cut tells if there is a superficial cut in A
-  *)
-  Fixpoint exp_done_rel A B : (bool * has_cut) :=
-    match A, B with
-    | Top, OK => (true, no)
-    | Goal _ Cut, OK => (true, sup)
-    | And A1 B01 B1, And A2 B02 B2 =>
-      if success A1 then 
-        let: (b1, hc) := exp_done_rel B1 B2 in
-        ((if hc == sup then (cutl A1 == A2) && (cutl B01 == B02)
-      else (A1 == A2) && (B01 == B02)) && b1, hc)
-      else 
-        let: (b1, hc) := exp_done_rel A1 A2 in
-        (b1 && (B01 == B02) && (B1 == B2),  hc)
-    | Or A1 _ B1, Or A2 _ B2 =>
-      if is_dead A1 then 
-        let: (b1, hc) := exp_done_rel B1 B2 in
-        ((A1 == A2) && b1, if hc == sup then deep else hc)
-      else 
-        let: (b1, hc) := exp_done_rel A1 A2 in 
-          (b1 && if hc == sup then cutr B1 == B2 else B1 == B2, if hc == sup then deep else hc)
-    | _, _ => (false, no)
-    end.
+    (*  
+      given two states A and B such that (exp_done_shape A),
+      returns (b * deep_cut * has_cut) where
+      - b tells if B is a valid evolution of A after a call to expand
+      - deep_cut tells a deep cut has been executed
+      - has_cut tells if there is a superficial cut in A
+    *)
+    Fixpoint exp_done_rel A B : (bool * has_cut) :=
+      match A, B with
+      | Top, OK => (true, no)
+      | Goal _ Cut, OK => (true, sup)
+      | And A1 B01 B1, And A2 B02 B2 =>
+        if success A1 then 
+          let: (b1, hc) := exp_done_rel B1 B2 in
+          ((if hc == sup then (cutl A1 == A2) && (cutl B01 == B02)
+        else (A1 == A2) && (B01 == B02)) && b1, hc)
+        else 
+          let: (b1, hc) := exp_done_rel A1 A2 in
+          (b1 && (B01 == B02) && (B1 == B2),  hc)
+      | Or A1 _ B1, Or A2 _ B2 =>
+        if is_dead A1 then 
+          let: (b1, hc) := exp_done_rel B1 B2 in
+          ((A1 == A2) && b1, if hc == sup then deep else hc)
+        else 
+          let: (b1, hc) := exp_done_rel A1 A2 in 
+            (b1 && if hc == sup then cutr B1 == B2 else B1 == B2, if hc == sup then deep else hc)
+      | _, _ => (false, no)
+      end.
 
-  Lemma exp_done_rel_success {A B hc}:
-    success A -> exp_done_rel A B = (true, hc) -> success B.
-  Proof.
-    elim: A B hc => //.
-    - move=> A HA s B HB []//A' s' B' hc/=.
-      case: ifP => [dA sB|dA sA]; case H: exp_done_rel => [[] hc'] //[]//.
-      - move=> /andP[/eqP<-];rewrite dA => _ _; apply: HB sB H.
-      - move=> /andP[]//.
-      - have sA' := (HA _ _ sA H); rewrite success_is_dead//.
-    - move=> A HA B0 _ B HB [] A' B0' B' // hc/= /andP[sA sB].
-      rewrite sA; case eB: exp_done_rel => [[] hc'][]/andP[]//.
-      case:ifP => /eqP?; subst => /andP[/eqP<- _ ?]; subst.
-      - rewrite success_cut//(HB _ _ sB eB)//.
-      - rewrite sA (HB _ _ sB eB)//.
-  Qed.
-
-  Lemma exp_done_shape_failed {A}: exp_done_shape A -> failed A = false.
-  Proof.
-    elim: A => //.
-    - move=> A HA s B HB/=; case: ifP => //.
-    - move=> A HA B0 _ B HB/=/andP[] /HA->/HB->; rewrite andbF//.
-  Qed.
-
-  Lemma exp_done_rel_dead {A B hc}: 
-    exp_done_rel A B = (true, hc) -> is_dead A = is_dead B.
-  Proof.
-    elim: A B hc => //.
-    - move=> []//.
-    - move=> p[]//=[]//.
-    - move=> A HA s B HB []//A' s' B' hc/=.
-      case: ifP => dA.
-        case X: exp_done_rel => [[] hc'][]/andP[]///eqP<- _.
-        rewrite dA (HB _ _ X)//.
-      case eA: exp_done_rel => //[[] hc']/=[]//.
-      case:ifP => /eqP?/eqP??; subst; rewrite -(HA _ _ eA) dA//.
-    - move=> A HA B0 _ B HB[]//A' B0' B' hc/=.
-      case: ifP => //sA; case H: exp_done_rel => [[] hc']//[]/andP[]//.
-        case:ifP => /eqP?; subst; move=>/andP[]/eqP<-; rewrite// is_dead_cutl//.
-      rewrite (HA _ _ H)//.
-  Qed.
-
-  Lemma exp_done_rel_failed {A B hc}: 
-    exp_done_rel A B = (true, hc) -> (failed A = false)%type.
-  Proof.
-    elim: A B hc => //.
-    - move=> A HA s B HB []//A' s' B' hc/=; case: ifP => dA.
-        case eB: exp_done_rel => [[] hc'][]/andP[]///eqP? _?; subst.
-        rewrite (HB _ _ eB)//.
-      case eA: exp_done_rel => [[] hc'][]//; subst.
-      rewrite (HA _ _ eA)//.
-    - move=> A HA B0 _ B HB/= []//A' B0' B' hc.
-      case: ifP => sA.
-        rewrite success_failed//=.
-        case eB: exp_done_rel => [[] hc'][]/andP[]//.
-        rewrite (HB _ _ eB)//.
-      case eA: exp_done_rel => [[] hc'][]//=.
-      rewrite (HA _ _ eA)//.
-  Qed.
-
-  Lemma exp_done_shape_big_or {p s t}: exp_done_shape (big_or p s t) = false.
-  Proof. rewrite/big_or; case: F => [|[]]//. Qed.
-
-  Lemma expand_exp_done_shape_cb {s1 A s2 B}: 
-    expand s1 A = CutBrothers s2 B -> exp_done_shape B -> 
-      (exp_done_rel A B) = (true, sup).
-  Proof.
-    elim: A s1 s2 B => //; auto.
-    - move=> p[|t]//=s1 s2 B [_<-]//.
-    - move=> A HA s B HB s1 s2 C/=.
-      case: ifP => //dA; case eB: expand => //[s1' B'][_<-]/=.
-      (* rewrite dA eqxx => H.
-      have -> := (HB _ _ _ eB H) => //. *)
-    - move=> A HA B0 _ B HB s1 s2 C/=.
-      case eA: expand => //[s3 D|s3 D].
-      - move=> [_<-]/=/andP[eD eB]; rewrite (expand_not_solved_not_success eA)//.
-        have:= HA _ _ _ eA eD.
-        case X: exp_done_rel => [b has_cut'][->->]; rewrite !eqxx//.
-      - case eB: expand => //[s4 E]/=[_ H1]/=; subst =>/= /andP[eD eE].
-        rewrite (expand_solved_success eA) (HB _ _ _ eB eE) (expand_solved_cutl eA) !eqxx//.
-  Qed.
-
-  Lemma expand_exp_done_shape_exp {s1 A s2 B}: 
-    expand s1 A = Expanded s2 B -> exp_done_shape B -> 
-      exists m, ((exp_done_rel A B = (true, m)) * ((m = no) \/ (m = deep)))%type.
-  Proof.
-    elim: A s1 s2 B => //; auto.
-    - move=> ??? [_<-]//=; eexists; auto.
-    - move=> p[|t]//=s1 s2 B [_<-]//.
-      rewrite exp_done_shape_big_or//.
-    - move=> A HA s B HB s1 s2 C/=.
-      case: ifP => //dA.
-        case eB: expand => // [s1' B'|s1' A'][_<-]/=; rewrite dA => H1.
-          have [m [H2 [H3|H3]]] := HB _ _ _ eB H1; rewrite eqxx H2 H3; eexists; auto.
-        rewrite (expand_exp_done_shape_cb eB H1) eqxx//=; eexists; auto.
-      case eA: expand => //[s1' A'|s1' A'] [_<-]/=; rewrite (expand_not_dead dA eA) => H1.
-        have [m [H2 [H3|H3]]] := HA _ _ _ eA H1; rewrite H2 eqxx H3//=; eexists; auto.
-      rewrite (expand_exp_done_shape_cb eA H1) !eqxx//; eexists; auto.
-    - move=> A HA B0 _ B HB s1 s2 C/=.
-      case eA: expand => //[s3 D|s3 D].
-      - move=> [_<-]/=/andP[eD eB]; rewrite (expand_not_solved_not_success eA)//.
-        have [m [H2 [H3|H3]]]:= HA _ _ _ eA eD; rewrite H2 H3/= !eqxx; eexists; auto.
-      - case eB: expand => //[s4 E]/=[_<-]/=/andP[eD eE].
-        have [m [H2 [H3|H3]]] := HB _ _ _ eB eE; rewrite H2 H3/= !eqxx;
-        rewrite (expand_solved_success eA) (expand_solved_same eA) !eqxx//; eexists; auto.
-  Qed.
-
-  Lemma exp_done_shapeP {s1 A s2 B b}: 
-    expandedb s1 A (Done s2 B) b -> exp_done_shape A.
-  Proof.
-    elim: A s1 s2 B b => //; try by inversion 1.
-    - move=>p [|t]// s1 s2 B b; inversion 1 => //; subst.
-      case: H1 => _ ?; subst; apply expandedb_big_or_not_done in H2 => //.
-    - move=> A HA s B HB s1 s2 C b H.
-      have /= := expandedb_same_structure H.
-      case: C H => //A' s' B' H /and3P[/eqP? _ _]; subst.
-      have:= expanded_or_complete H => -[][]->.
-        move=> [b1[H1 ?]]; subst; apply: HA H1.
-      move=> [? [b1 H1]]; subst; apply: HB H1.
-    - move=> A HA B0 _ B HB s1 s2 C b H.
-      have /= := expandedb_same_structure H.
-      case: C H => //A' s' B' H _; subst.
-      have [s''[A1[B1[b1[b2[H1[H2 H3]]]]]]]:= expanded_and_complete H; subst.
-      by rewrite (HA _ _ _ _ H1) (HB _ _ _ _ H2).
-  Qed.
-
-  (* Lemma exp_done_rel_bool {A B b1 b2}: 
-    exp_done_rel A B = (b1, b2, true) -> 
-      ((b2 = true))%type.
-  Proof.
-    elim: A B b1 b2 => //.
-    - move=> []//.
-    - move=> p[]//[]// b1[]//=.
-    - move=> A HA s B HB []//A' s' B' b1 b2/=.
-      case: ifP => //dA.
-        case eB: exp_done_rel => [[b1' b2'] b3'][] H1 H2 H3//; subst.
-      case eA: exp_done_rel => [[b1' b2'] b3'][] H1 H2 H3; subst => //.
-    - move=> A HA B0 _ B HB[]//A' B0' B' b1 b2//=.
-      case: ifP => // sA.
-        case eB: exp_done_rel => [[b1' b2'] b3'][] H1 H2 H3; subst.
-        have H := HB _ _ _ eB; rewrite !H//.
-      case eA: exp_done_rel => [[b1' b2'] b3'][] H1 H2 H3; subst => //.
-      have H := HA _ _ _ eA.
-      rewrite !H//.
-  Qed.
-
-  Lemma exp_done_rel_bool1 {A B b1 b2}: 
-    exp_done_rel A B = (b1, false, b2) -> 
-      ((b2 = false))%type.
-  Proof.
-    elim: A B b1 b2 => //.
-    - move=>/= _ []//[]//.
-    - move=>/= _ []//[]//.
-    - move=> /= B; case X: B => ??[??]//.
-    - move=>/= _ []//[]//.
-    - move=> p[|t]//= B b1 b2.
-        case C: B => //-[??]//.
-      move=>[]//.
-    - move=> A HA s B HB C b1 b2.
-      case HC: C => /=; last first; [ | | try by move=>[]..].
-        move=> []//.
-      case: ifP => //dA.
-        case eB: exp_done_rel => [[b1' b2'] b3'][] H1 H2 H3//; subst.
-      case eA: exp_done_rel => [[b1' b2'] b3'][] H1 H2 H3; subst => //.
-    - move=> A HA B0 _ B HB C b1 b2.
-      case HC: C => //=; last first; [| move=> []//..].
-      case: ifP => // sA.
-        case eB: exp_done_rel => [[b1' b2'] b3'][]+??; subst.
-        by have:= HB _ _ _ eB.
-      case eA: exp_done_rel => [[b1' b2'] b3'][] H1 H2 H3; subst => //.
-      by have H := HA _ _ _ eA.
-  Qed.
-  Print lvl0. *)
-
-  Definition empty_ca A := match A with cut _ [::] | call _ _ => true | _ => false end.
-  Definition all_empty_ca := all empty_ca.
-
-  Lemma exp_done_rel_txt_state_to_list {B B'} l1:
-    valid_state B ->
-    exp_done_rel B B' = (true, sup) ->
-      exists xs tl, state_to_list B l1 = [::[::cut true [::] & xs] & tl].
-  Proof.
-    elim: B B' l1 => //.
-    - move=> []//.
-    - move=> p[]//[]//l1/=; by do 2 eexists.
-    - move=> A HA s B HB[]//A' s' B' l1/=.
-      case: ifP => [dA vB|dA /andP[vA bB]]; case eB: exp_done_rel => [[] []][]//.
-    - move=> A HA B0 _ B HB []//A' B0' B' l1/=/and5P[oA vA AB].
-      case: ifP => /=[sA vB bB0 |sA /eqP->].
-        case eB: exp_done_rel => [[] []][]///andP[]///andP[/eqP?/eqP?] _; subst.
-        rewrite (success_state_to_list sA) add_alt_empty1 /=.
-        have [xs[tl H]]:= (HB _ l1 vB eB).
-        rewrite H; by do 2 eexists.
-      case eA: exp_done_rel => [[] []]//.
-      rewrite (exp_done_rel_failed eA)=> bB[]/andP[/eqP?/eqP?]; subst.
-      have [hd->]:= base_and_state_to_list bB.
-      have [xs[tl ->]]:= HA _ l1 vA eA.
-      by do 2 eexists.
-    Qed.
-
-  Lemma xxx {B B' l1 l2}:
-    exp_done_shape B' ->
-    exp_done_rel B B' = (true, no) ->
-     map (map (add_ca l1)) (state_to_list B' l2) = state_to_list B' l2.
-  Proof.
-    Abort.
-
-  Lemma exp_done_rel_tfx {A B} l:
-    valid_state A -> exp_done_shape B -> exp_done_rel A B = (true, no) ->
-      state_to_list A l = state_to_list B l.
-  Proof.
-    elim: A B l => //.
-    - move=> []//.
-    - move=> /= p [|t]// []//= m _ _ _.
-    - move=> A HA s B HB []//A' s' B' l1/=.
-      case: ifP => [dA vB|dA/andP[vA bB]] HH.
-        case eB: exp_done_rel => [[] []][]/andP[]///eqP? _; subst.
-        rewrite dA in HH.
-        rewrite (HB _ _ vB HH eB)//.
-      case eA: exp_done_rel => [[] []][]///eqP?; subst.
-      rewrite -(exp_done_rel_dead eA)dA in HH.
-      rewrite (HA _ _ vA HH eA)//.
-    - move=> A HA B0 _ B HB []//A' B0' B'/=l1 /and5P[oA vA aB].
-      case: ifP => /=[sA vB bB0 /andP[xA xB]|sA /eqP->].
-        case eB: exp_done_rel => [[] []][]///andP[]///andP[/eqP?/eqP?]? ; subst.
-        rewrite (success_state_to_list sA).
-        rewrite !add_alt_empty1.
-        have H:= HB _ _ vB xB eB.
-        rewrite H//.
-      case eA: exp_done_rel => [[] []]//; rewrite (exp_done_rel_failed eA).
-      move=> bB /andP[xA xB] [] /andP[/eqP?/eqP?]; subst.
-      rewrite (HA _ l1 vA xA eA)//.
-  Qed.
-
-  Section lvlF.
-    Definition lvlF A := match A with cut b1 _ => ~~b1 | _ => true end.
-
-    Lemma lvlF_incr {x}: lvlF x -> incr_cut x = x.
-    Proof. case: x => //-[]//. Qed.
-
-    Lemma all_lvlF_incr {ca}:
-      all lvlF ca -> map incr_cut ca = ca.
-    Proof. elim: ca => //x xs IH/=/andP[H1 H2]; rewrite IH//lvlF_incr//. Qed.
-
-    Lemma all2_lvlF_incr {ca}:
-      all (all lvlF) ca -> incr_cuts ca = ca.
+    Lemma exp_done_rel_success {A B hc}:
+      success A -> exp_done_rel A B = (true, hc) -> success B.
     Proof.
-      elim: ca => //x xs IH/=/andP[] H1 H2.
-      rewrite IH//all_lvlF_incr//.
+      elim: A B hc => //.
+      - move=> A HA s B HB []//A' s' B' hc/=.
+        case: ifP => [dA sB|dA sA]; case H: exp_done_rel => [[] hc'] //[]//.
+        - move=> /andP[/eqP<-];rewrite dA => _ _; apply: HB sB H.
+        - move=> /andP[]//.
+        - have sA' := (HA _ _ sA H); rewrite success_is_dead//.
+      - move=> A HA B0 _ B HB [] A' B0' B' // hc/= /andP[sA sB].
+        rewrite sA; case eB: exp_done_rel => [[] hc'][]/andP[]//.
+        case:ifP => /eqP?; subst => /andP[/eqP<- _ ?]; subst.
+        - rewrite success_cut//(HB _ _ sB eB)//.
+        - rewrite sA (HB _ _ sB eB)//.
     Qed.
 
-    Lemma lvlF_incrT {x}: lvlF (incr_cut x).
-    Proof. case: x => //-[]//. Qed.
-
-    Lemma all_lvlF_incrT {ca}:
-      all lvlF (map incr_cut ca).
-    Proof. elim: ca => // x xs/=->; rewrite lvlF_incrT//. Qed.
-
-    Lemma all2_lvlF_incrT {ca}:
-      all (all lvlF) (incr_cuts ca).
-    Proof. elim: ca => // x xs/=->; rewrite all_lvlF_incrT//. Qed.
-
-    Lemma lvlF_base_and_ko_s2l {B l}:
-      base_and_ko B -> all (all lvlF) l -> all (all lvlF) (state_to_list B l).
-    Proof. elim: B l => //=-[]//. Qed.
-
-    Lemma lvlF_base_or_ko_s2l {B l}:
-      base_or_aux_ko B -> all (all lvlF) l -> all (all lvlF) (state_to_list B l).
-    Proof. 
-      elim: B l => //.
-        move=> A HA s B HB l/=/andP[bA bB] H.
-        rewrite all2_lvlF_incrT//.
-      move=> []//.
+    Lemma exp_done_shape_failed {A}: exp_done_shape A -> failed A = false.
+    Proof.
+      elim: A => //.
+      - move=> A HA s B HB/=; case: ifP => //.
+      - move=> A HA B0 _ B HB/=/andP[] /HA->/HB->; rewrite andbF//.
     Qed.
 
-    Lemma lvlF_add_ca {ca x}: lvlF ca -> lvlF (add_ca x ca).
-    Proof. case: ca => //. Qed.
+    Lemma exp_done_rel_dead {A B hc}: 
+      exp_done_rel A B = (true, hc) -> is_dead A = is_dead B.
+    Proof.
+      elim: A B hc => //.
+      - move=> []//.
+      - move=> p[]//=[]//.
+      - move=> A HA s B HB []//A' s' B' hc/=.
+        case: ifP => dA.
+          case X: exp_done_rel => [[] hc'][]/andP[]///eqP<- _.
+          rewrite dA (HB _ _ X)//.
+        case eA: exp_done_rel => //[[] hc']/=[]//.
+        case:ifP => /eqP?/eqP??; subst; rewrite -(HA _ _ eA) dA//.
+      - move=> A HA B0 _ B HB[]//A' B0' B' hc/=.
+        case: ifP => //sA; case H: exp_done_rel => [[] hc']//[]/andP[]//.
+          case:ifP => /eqP?; subst; move=>/andP[]/eqP<-; rewrite// is_dead_cutl//.
+        rewrite (HA _ _ H)//.
+    Qed.
 
-    Lemma all_lvlF_add_ca {ca x}: (all lvlF) ca -> (all lvlF) ((map (add_ca x)) ca).
-    Proof. elim: ca x => //x xs IH y/=/andP[H1 H2]; rewrite IH//lvlF_add_ca//. Qed.
+    Lemma exp_done_rel_failed {A B hc}: 
+      exp_done_rel A B = (true, hc) -> (failed A = false)%type.
+    Proof.
+      elim: A B hc => //.
+      - move=> A HA s B HB []//A' s' B' hc/=; case: ifP => dA.
+          case eB: exp_done_rel => [[] hc'][]/andP[]///eqP? _?; subst.
+          rewrite (HB _ _ eB)//.
+        case eA: exp_done_rel => [[] hc'][]//; subst.
+        rewrite (HA _ _ eA)//.
+      - move=> A HA B0 _ B HB/= []//A' B0' B' hc.
+        case: ifP => sA.
+          rewrite success_failed//=.
+          case eB: exp_done_rel => [[] hc'][]/andP[]//.
+          rewrite (HB _ _ eB)//.
+        case eA: exp_done_rel => [[] hc'][]//=.
+        rewrite (HA _ _ eA)//.
+    Qed.
 
-    Lemma all2_lvlF_add_ca {ca x}: all (all lvlF) ca -> all (all lvlF) (map (map (add_ca x)) ca).
-    Proof. elim: ca x => //x xs IH y/=/andP[H1 H2]; rewrite IH//all_lvlF_add_ca//. Qed.
+    Lemma exp_done_shape_big_or {p s t}: exp_done_shape (big_or p s t) = false.
+    Proof. rewrite/big_or; case: F => [|[]]//. Qed.
 
-  End lvlF.
+    Lemma expand_exp_done_shape_cb {s1 A s2 B}: 
+      expand s1 A = CutBrothers s2 B -> exp_done_shape B -> 
+        (exp_done_rel A B) = (true, sup).
+    Proof.
+      elim: A s1 s2 B => //; auto.
+      - move=> p[|t]//=s1 s2 B [_<-]//.
+      - move=> A HA s B HB s1 s2 C/=.
+        case: ifP => //dA; case eB: expand => //[s1' B'][_<-]/=.
+        (* rewrite dA eqxx => H.
+        have -> := (HB _ _ _ eB H) => //. *)
+      - move=> A HA B0 _ B HB s1 s2 C/=.
+        case eA: expand => //[s3 D|s3 D].
+        - move=> [_<-]/=/andP[eD eB]; rewrite (expand_not_solved_not_success eA)//.
+          have:= HA _ _ _ eA eD.
+          case X: exp_done_rel => [b has_cut'][->->]; rewrite !eqxx//.
+        - case eB: expand => //[s4 E]/=[_ H1]/=; subst =>/= /andP[eD eE].
+          rewrite (expand_solved_success eA) (HB _ _ _ eB eE) (expand_solved_cutl eA) !eqxx//.
+    Qed.
 
-  Lemma expand_exp_state_to_list1 {s1 A s2 A' s}:
-    expand s1 A = Expanded s2 A' -> exp_done_rel A A' = (true, s) -> s <> sup.
-  Proof.
-    elim: A A' s1 s => //.
-    - move=>[]// ?? _ [<-]//.
-    - move=> p[]//.
-    - move=> A HA s B HB/= []//A' s' B' s1 s3.
-      case:ifP => dA; case X: exp_done_rel => [[] []]+[]// H1 H2; subst => //.
-    - move=> A HA B0 _ B HB[]//A' B0' B' s1 s/=.
-      case eA: expand => //[s1' A2|s1' A2].
-        move=>[????]; subst.
-        rewrite (expand_not_solved_not_success eA erefl) .
-        case H1: exp_done_rel => [[] X][]///andP[]*; subst.
-        apply: HA eA H1.
-      case eB: expand => //[s3 B2][????]; subst.
-      rewrite (expand_solved_success eA).
-      case H1: exp_done_rel => [[] X][]/andP[]// _ _ <-.
-      apply: HB eB H1.
-  Qed.
+    Lemma expand_exp_done_shape_exp {s1 A s2 B}: 
+      expand s1 A = Expanded s2 B -> exp_done_shape B -> 
+        exists m, ((exp_done_rel A B = (true, m)) * ((m = no) \/ (m = deep)))%type.
+    Proof.
+      elim: A s1 s2 B => //; auto.
+      - move=> ??? [_<-]//=; eexists; auto.
+      - move=> p[|t]//=s1 s2 B [_<-]//.
+        rewrite exp_done_shape_big_or//.
+      - move=> A HA s B HB s1 s2 C/=.
+        case: ifP => //dA.
+          case eB: expand => // [s1' B'|s1' A'][_<-]/=; rewrite dA => H1.
+            have [m [H2 [H3|H3]]] := HB _ _ _ eB H1; rewrite eqxx H2 H3; eexists; auto.
+          rewrite (expand_exp_done_shape_cb eB H1) eqxx//=; eexists; auto.
+        case eA: expand => //[s1' A'|s1' A'] [_<-]/=; rewrite (expand_not_dead dA eA) => H1.
+          have [m [H2 [H3|H3]]] := HA _ _ _ eA H1; rewrite H2 eqxx H3//=; eexists; auto.
+        rewrite (expand_exp_done_shape_cb eA H1) !eqxx//; eexists; auto.
+      - move=> A HA B0 _ B HB s1 s2 C/=.
+        case eA: expand => //[s3 D|s3 D].
+        - move=> [_<-]/=/andP[eD eB]; rewrite (expand_not_solved_not_success eA)//.
+          have [m [H2 [H3|H3]]]:= HA _ _ _ eA eD; rewrite H2 H3/= !eqxx; eexists; auto.
+        - case eB: expand => //[s4 E]/=[_<-]/=/andP[eD eE].
+          have [m [H2 [H3|H3]]] := HB _ _ _ eB eE; rewrite H2 H3/= !eqxx;
+          rewrite (expand_solved_success eA) (expand_solved_same eA) !eqxx//; eexists; auto.
+    Qed.
 
-  (* Lemma expand_exp_state_lvlF {s1 A s2 A' l x ca'}:
-    valid_state A -> expand s1 A = Expanded s2 A' -> (state_to_list A' l = x :: ca') -> all (all lvlF) ca'.
-  Proof.
-    elim: A A' s1 s2 l x ca' => //.
-    - move=> []// s1 s2 l x ca' _ /=[?][_<-]//.
-    - move=> p[]//t A' s1 s2 x c ca' _/=[_<-];rewrite/big_or.
-      case: F=>//-[y ys]l/=.
-      case: state_to_list => //[z zs]/=[??]; subst.
-      apply: all2_lvlF_incrT.
-    - move=> A HA s B HB C s1 s2 l x ca'/=.
-      case: ifP => [dA vB|da /andP[va bB]].
-        case eB:expand => //[s1' B'|s1' B'][??]; subst => /=; rewrite (state_to_list_dead dA)/=;
-        case: state_to_list => //[y ys][_<-]; apply: all2_lvlF_incrT.
-      case eA: expand => //[s1' A'|s1' A'][_<-]/=; case: cat => //[w ws][_<-]; apply: all2_lvlF_incrT.
-    - move=> A HA B0 _ B HB/= C s1 s2 l x ca/and5P[oA vA aB].
-      case eA: expand => //[s1' A2|s1' A2].
-        rewrite (expand_not_solved_not_success eA erefl) (expand_not_failed eA notF)/=.
-        move=>/eqP->bB[_<-]/=.
-        case sA: state_to_list => //[w ws].
-        have [hd H]:= base_and_state_to_list bB.
-        have Hw := HA _ _ _ _ _ _ vA eA sA.
-        rewrite H=>-[H1 H2]; rewrite -H2/make_lB0/=.
+    Lemma exp_done_shapeP {s1 A s2 B b}: 
+      expandedb s1 A (Done s2 B) b -> exp_done_shape A.
+    Proof.
+      elim: A s1 s2 B b => //; try by inversion 1.
+      - move=>p [|t]// s1 s2 B b; inversion 1 => //; subst.
+        case: H1 => _ ?; subst; apply expandedb_big_or_not_done in H2 => //.
+      - move=> A HA s B HB s1 s2 C b H.
+        have /= := expandedb_same_structure H.
+        case: C H => //A' s' B' H /and3P[/eqP? _ _]; subst.
+        have:= expanded_or_complete H => -[][]->.
+          move=> [b1[H1 ?]]; subst; apply: HA H1.
+        move=> [? [b1 H1]]; subst; apply: HB H1.
+      - move=> A HA B0 _ B HB s1 s2 C b H.
+        have /= := expandedb_same_structure H.
+        case: C H => //A' s' B' H _; subst.
+        have [s''[A1[B1[b1[b2[H1[H2 H3]]]]]]]:= expanded_and_complete H; subst.
+        by rewrite (HA _ _ _ _ H1) (HB _ _ _ _ H2).
+    Qed.
 
-        have:
-
-        move=>[????]; subst.
-        have [b1[b2 H]]:= HA _ _ eA.
-        rewrite H (expand_not_solved_not_success eA erefl).
+    Lemma exp_done_rel_txt_state_to_list {B B'} l1:
+      valid_state B ->
+      exp_done_rel B B' = (true, sup) ->
+        exists xs tl, state_to_list B l1 = [::[::cut false [::] & xs] & tl].
+    Proof.
+      elim: B B' l1 => //.
+      - move=> []//.
+      - move=> p[]//[]//l1/=; by do 2 eexists.
+      - move=> A HA s B HB[]//A' s' B' l1/=.
+        case: ifP => [dA vB|dA /andP[vA bB]]; case eB: exp_done_rel => [[] []][]//.
+      - move=> A HA B0 _ B HB []//A' B0' B' l1/=/and5P[oA vA AB].
+        case: ifP => /=[sA vB bB0 |sA /eqP->].
+          case eB: exp_done_rel => [[] []][]///andP[]///andP[/eqP?/eqP?] _; subst.
+          rewrite (success_state_to_list sA) add_alt_empty1 /=.
+          have [xs[tl H]]:= (HB _ l1 vB eB).
+          rewrite H; by do 2 eexists.
+        case eA: exp_done_rel => [[] []]//.
+        rewrite (exp_done_rel_failed eA)=> bB[]/andP[/eqP?/eqP?]; subst.
+        have [hd->]:= base_and_state_to_list bB.
+        have [xs[tl ->]]:= HA _ l1 vA eA.
         by do 2 eexists.
-      case eB: expand => //[s3 B2][????]; subst.
-      have [b1[b2 H]]:= HB _ _ eB.
-      rewrite H (expand_solved_success eA).
-      by do 2 eexists.
-  Qed. *)
+      Qed.
 
-  Lemma bibi1 {A B s s'} l:
-    valid_state A -> exp_done_shape B -> exp_done_rel A B = (true, deep) ->
-      expand s A = Expanded s' B ->
-      exists x tl ca r, 
-        (((state_to_list A l = [:: [::cut false ca & x] & tl]) * 
-          (state_to_list B l = [::x & r])) * 
-            (r = ca \/ r = incr_cuts ca \/ r = [::])
-          (* * all (all lvlF) ca *)
-          )%type.
-  Proof.
-    elim: A B s s' l => //.
-    - move=> []//.
-    - move=> p []//[]//.
-    - move=> A HA s B HB[]//A' s' B' s1 s2 l/=.
-      case: ifP => [dA vB|dA /andP[vA bB]] H.
-        (* dead A \/ B *)
-        rewrite !(state_to_list_dead dA)/=.
-        case eB: exp_done_rel => [[] []][]///andP[]///eqP? _; subst; rewrite dA in H; rewrite (state_to_list_dead dA)/=.
-          have [xs[tl H1]]:= exp_done_rel_txt_state_to_list l vB eB; rewrite H1/=.
-          case eA:expand => //[s1' B2|s1' B2][??]?; subst.
-            by have := (expand_exp_state_to_list1 eA eB).
-          have [x[tl0 [+ lx]]]:= expand_cb_state_to_list1 l vB eA.
-          move=>/(_ l)[]; rewrite H1 => -[??] H2; subst.
-          rewrite H2/=.
-          do 4 eexists; auto.
-          (* exists [::], [::] => //. *)
-        case EB: expand => //[s1' B2|s1' B2][??]?; subst.
-          have [x[tl[ca[r[H1 [|[]]]]]]]:= HB _ _ _ l vB H eB EB; rewrite !H1 => ?/=; subst;
+    Lemma xxx {B B' l1 l2}:
+      exp_done_shape B' ->
+      exp_done_rel B B' = (true, no) ->
+      map (map (add_ca false l1)) (state_to_list B' l2) = state_to_list B' l2.
+    Proof.
+      Abort.
+
+    Lemma exp_done_rel_tfx {A B} l:
+      valid_state A -> exp_done_shape B -> exp_done_rel A B = (true, no) ->
+        state_to_list A l = state_to_list B l.
+    Proof.
+      elim: A B l => //.
+      - move=> []//.
+      - move=> /= p [|t]// []//= m _ _ _.
+      - move=> A HA s B HB []//A' s' B' l1/=.
+        case: ifP => [dA vB|dA/andP[vA bB]] HH.
+          case eB: exp_done_rel => [[] []][]/andP[]///eqP? _; subst.
+          rewrite dA in HH.
+          rewrite (HB _ _ vB HH eB)//.
+        case eA: exp_done_rel => [[] []][]///eqP?; subst.
+        rewrite -(exp_done_rel_dead eA)dA in HH.
+        rewrite (HA _ _ vA HH eA)//.
+      - move=> A HA B0 _ B HB []//A' B0' B'/=l1 /and5P[oA vA aB].
+        case: ifP => /=[sA vB bB0 /andP[xA xB]|sA /eqP->].
+          case eB: exp_done_rel => [[] []][]///andP[]///andP[/eqP?/eqP?]? ; subst.
+          rewrite (success_state_to_list sA).
+          rewrite !add_alt_empty1.
+          have H:= HB _ _ vB xB eB.
+          rewrite H//.
+        case eA: exp_done_rel => [[] []]//; rewrite (exp_done_rel_failed eA).
+        move=> bB /andP[xA xB] [] /andP[/eqP?/eqP?]; subst.
+        rewrite (HA _ l1 vA xA eA)//.
+    Qed.
+
+    Lemma expand_exp_state_to_list1 {s1 A s2 A' s}:
+      expand s1 A = Expanded s2 A' -> exp_done_rel A A' = (true, s) -> s <> sup.
+    Proof.
+      elim: A A' s1 s => //.
+      - move=>[]// ?? _ [<-]//.
+      - move=> p[]//.
+      - move=> A HA s B HB/= []//A' s' B' s1 s3.
+        case:ifP => dA; case X: exp_done_rel => [[] []]+[]// H1 H2; subst => //.
+      - move=> A HA B0 _ B HB[]//A' B0' B' s1 s/=.
+        case eA: expand => //[s1' A2|s1' A2].
+          move=>[????]; subst.
+          rewrite (expand_not_solved_not_success eA erefl) .
+          case H1: exp_done_rel => [[] X][]///andP[]*; subst.
+          apply: HA eA H1.
+        case eB: expand => //[s3 B2][????]; subst.
+        rewrite (expand_solved_success eA).
+        case H1: exp_done_rel => [[] X][]/andP[]// _ _ <-.
+        apply: HB eB H1.
+    Qed.
+
+    Lemma bibi1 {A B s s'} l:
+      valid_state A -> exp_done_shape B -> exp_done_rel A B = (true, deep) ->
+        expand s A = Expanded s' B ->
+        exists x tl ca r, 
+          (((state_to_list A l = [:: [::cut true ca & x] & tl]) * 
+            (state_to_list B l = [::x & r])) * 
+              (r = ca \/ r = incr_cuts ca)
+            (* * all (all lvlD) ca *)
+            )%type.
+    Proof.
+      elim: A B s s' l => //.
+      - move=> []//.
+      - move=> p []//[]//.
+      - move=> A HA s B HB[]//A' s' B' s1 s2 l/=.
+        case: ifP => [dA vB|dA /andP[vA bB]] H.
+          (* dead A \/ B *)
+          rewrite !(state_to_list_dead dA)/=.
+          case eB: exp_done_rel => [[] []][]///andP[]///eqP? _; subst; rewrite dA in H; rewrite (state_to_list_dead dA)/=.
+            have [xs[tl H1]]:= exp_done_rel_txt_state_to_list l vB eB; rewrite H1/=.
+            case eA:expand => //[s1' B2|s1' B2][??]?; subst.
+              by have := (expand_exp_state_to_list1 eA eB).
+            have [x[tl0 [+ lx]]]:= expand_cb_state_to_list1 l vB eA.
+            move=>/(_ l)[]; rewrite H1 => -[??] H2; subst.
+            rewrite H2/=.
             do 4 eexists; auto.
-          repeat split; auto; rewrite incr_cuts2; auto.
-          (* exists ca, (incr_cuts ca') => //. *)
-          (* rewrite all2_lvlF_incr//. *)
-        by rewrite (expand_exp_done_shape_cb EB H) in eB.
-      case eA: exp_done_rel => [[] h][]//.
-      case EA:expand => //[s1' A2|s1' A2] + + [??]??; subst; rewrite (expand_not_dead dA EA) in H.
-        have H1 := expand_exp_state_to_list1 EA eA.
-        case: h H1 eA => // _ eA/=/eqP _ _.
-        have [x[tl[ca[ca'[H1 [|[]]]]]]]:= HA _ _ _ (state_to_list B' l ++ l) vA H eA EA => ?; subst; rewrite 2!H1/=.
-        - do 4 eexists; repeat split. admit.
-        - do 4 eexists; repeat split. admit.
-        - do 4 eexists; repeat split. admit.
-        (* do 2 eexists. *)
-        (* exists (ca++l), (incr_cuts (map (map (add_ca l)) ca' ++ state_to_list B' l)) => //; auto. *)
-      have:= (expand_exp_done_shape_cb EA H); rewrite eA => -[?]; subst.
-      have [x[tl [H2 H3]]]:= expand_cb_state_to_list1 ((state_to_list B l ++ l)) vA EA.
-      have vB:= bbOr_valid bB => /= _ _.
-      rewrite !(H2 (state_to_list (cutr B) l ++ l))/=.
-      rewrite state_to_list_cutr_empty//=.
-      (* eexists; exists [::]. *)
-      do 2 eexists.
-      do 2 eexists; split => //; auto.
-      (* repeat split; f_equal. *)
-    - move=> A HA B0 _ B HB []//A' B0' B' s s' l/=/and5P[oA vA aB].
-      case eA: expand => //[s2 A2|s2 A2].
-        rewrite (expand_not_solved_not_success eA erefl)(expand_not_failed eA notF)/=.
-        move=>/eqP->bB/andP[xA xB].
-        have [hd H]:= base_and_state_to_list bB.
-        have H3 := base_and_lvl0 bB (H [::]).
-        case bA: exp_done_rel => [[] hc][]///andP[/eqP?/eqP?]?[????]; subst.
-        have [x[tl[ca[ca' [{}HA Hm]]]]]:= HA _ _ _ l vA xA bA eA.
-        rewrite 2!HA.
-        rewrite H.
-        rewrite/add_alt/make_lB/make_lB0/=.
-        rewrite 2!(all_lvl0_add_ca0 H3).
+            (* exists [::], [::] => //. *)
+          case EB: expand => //[s1' B2|s1' B2][??]?; subst.
+            have [x[tl[ca[r[H1 []]]]]]:= HB _ _ _ l vB H eB EB; rewrite !H1 => ?/=; subst;
+              do 4 eexists; auto.
+            repeat split; auto; rewrite incr_cuts2; auto.
+            (* exists ca, (incr_cuts ca') => //. *)
+            (* rewrite all2_lvlF_incr//. *)
+          by rewrite (expand_exp_done_shape_cb EB H) in eB.
+        case eA: exp_done_rel => [[] h][]//.
+        case EA:expand => //[s1' A2|s1' A2] + + [??]??; subst; rewrite (expand_not_dead dA EA) in H.
+          have H1 := expand_exp_state_to_list1 EA eA.
+          case: h H1 eA => // _ eA/=/eqP _ _.
+          have [x[tl[ca[ca'[H1 []]]]]]:= HA _ _ _ (state_to_list B' l ++ l) vA H eA EA => ?; subst; rewrite 2!H1/=.
+          - admit.
+          - admit.
+          (* do 2 eexists. *)
+          (* exists (ca++l), (incr_cuts (map (map (add_ca l)) ca' ++ state_to_list B' l)) => //; auto. *)
+        have:= (expand_exp_done_shape_cb EA H); rewrite eA => -[?]; subst.
+        have [x[tl [H2 H3]]]:= expand_cb_state_to_list1 ((state_to_list B l ++ l)) vA EA.
+        have vB:= bbOr_valid bB => /= _ _.
+        rewrite !(H2 (state_to_list (cutr B) l ++ l))/=.
+        rewrite state_to_list_cutr_empty//=.
+        (* eexists; exists [::]. *)
         do 2 eexists.
-        eexists ca, (flatten [seq [:: la ++ hd] | la <- ca']) => //.
+        do 2 eexists; split => //; auto.
         admit.
-      rewrite (expand_solved_success eA)/==>vB bB/andP[xA' xB'].
-      case eB: exp_done_rel => [[] hc][] /andP[]// +??; subst.
-      move=>/andP[/eqP?/eqP?]; subst.
-      have [??] := expand_solved_same eA; subst.
-      have [sA _] := expand_solved_success eA; subst.
-      rewrite (success_state_to_list sA)!add_alt_empty1.
-      case EB: expand => //[s2' B2][??]; subst.
-      have [x[tl[ca[ca'[H1 H2]]]]]:= HB _ _ _ l vB xB' eB EB.
-      rewrite !H1/=.
-      move: bB; rewrite/bbAnd=>/orP[]bB; last first.
-        rewrite (base_and_ko_state_to_list bB) !make_lB0_empty2 !cats0 !add_ca0_empty.
-        rewrite make_lB_empty2 make_lB_empty2.
-        do 2 eexists.
-        exists ca, ca' => //.
-      have [hd H3] := base_and_state_to_list bB.
-      rewrite H3/make_lB0/=.
-      do 2 eexists => //.
-      exists 
-        (ca ++ flatten [seq [:: la ++ hd] | la <- state_to_list (clean_success A2) l]),
-      (make_lB ca'
-        (flatten [seq [:: la ++ hd] | la <- state_to_list (clean_success A2) l]) ++
-        flatten [seq [:: la ++ hd] | la <- state_to_list (clean_success A2) l]) => //.
-      admit.
-  Admitted.
-
-  Lemma same_subst (s1 s2: Sigma): s1 = s2. Admitted.
+        (* repeat split; f_equal. *)
+      - move=> A HA B0 _ B HB []//A' B0' B' s s' l/=/and5P[oA vA aB].
+        case eA: expand => //[s2 A2|s2 A2].
+          rewrite (expand_not_solved_not_success eA erefl)(expand_not_failed eA notF)/=.
+          move=>/eqP->bB/andP[xA xB].
+          have [hd H]:= base_and_state_to_list bB.
+          have H3 := base_and_lvlt bB (H [::]).
+          case bA: exp_done_rel => [[] hc][]///andP[/eqP?/eqP?]?[????]; subst.
+          have [x[tl[ca[ca' [{}HA Hm]]]]]:= HA _ _ _ l vA xA bA eA.
+          rewrite 2!HA.
+          rewrite H.
+          rewrite/add_alt/make_lB/make_lB0/=.
+          rewrite 2!(all_lvlt_add_caF H3).
+          do 2 eexists.
+          eexists ca, (flatten [seq [:: la ++ hd] | la <- ca']) => //.
+          admit.
+        rewrite (expand_solved_success eA)/==>vB bB/andP[xA' xB'].
+        case eB: exp_done_rel => [[] hc][] /andP[]// +??; subst.
+        move=>/andP[/eqP?/eqP?]; subst.
+        have [??] := expand_solved_same eA; subst.
+        have [sA _] := expand_solved_success eA; subst.
+        rewrite (success_state_to_list sA)!add_alt_empty1.
+        case EB: expand => //[s2' B2][??]; subst.
+        have [x[tl[ca[ca'[H1 H2]]]]]:= HB _ _ _ l vB xB' eB EB.
+        rewrite !H1/=.
+        move: bB; rewrite/bbAnd=>/orP[]bB; last first.
+          rewrite (base_and_ko_state_to_list bB) !make_lB0_empty2 !cats0 !add_ca_empty.
+          rewrite make_lB_empty2 make_lB_empty2.
+          do 2 eexists.
+          exists ca, ca' => //.
+        have [hd H3] := base_and_state_to_list bB.
+        rewrite H3/make_lB0/=.
+        do 2 eexists => //.
+        exists 
+          (ca ++ flatten [seq [:: la ++ hd] | la <- state_to_list (clean_success A2) l]),
+        (make_lB ca'
+          (flatten [seq [:: la ++ hd] | la <- state_to_list (clean_success A2) l]) ++
+          flatten [seq [:: la ++ hd] | la <- state_to_list (clean_success A2) l]) => //.
+        admit.
+    Admitted.
+  End exp_done_rel.
 
   (* In this lemma, we do not backtrack: the solution is found
      in a given subtree, therefore we can state_to_list with any bt list
@@ -1879,7 +1885,7 @@ Module Nur (U : Unif).
     remember (Done _ _) as d eqn:Hd => + H.
     elim: H s' B Hd => //; clear.
     - move=> s s' A A' + s1 B [??] _; subst.
-      apply: expand_done.
+      apply: expand_solved.
     - move=> s s' r A B b HA HB IH s1 C ? vA; subst.
       have {IH} := IH _ _ erefl (valid_state_expand vA HA).
       have [x[xs sA]]:= expand_state_to_list_cons vA HA notF [::].
@@ -1903,11 +1909,136 @@ Module Nur (U : Unif).
       have [x1[ca[tl[ca']]]] := bibi1 [::] vA eB eA HA.
       rewrite sA sB=> -[][][??][??]; subst.
       rewrite (same_subst s s')//.
-      move=>[|[]]?; subst; apply: CutE.
+      move=>[]?; subst; apply: CutE.
       - auto.
       - admit. (*questo è accettabile: la nur non usa il bool *)
-      - admit. 
   Admitted.
+
+  Lemma expandedb_failure_next_alt_state_to_list_cons1 {s1 A B b1} l:
+    valid_state A -> expandedb s1 A (Failed B) b1 -> 
+    state_to_list A l = state_to_list B l (* reached a Bot *)
+      \/ 
+      (exists hd p t tl gl, 
+        state_to_list A l = (hd ++ call p t :: tl) :: gl /\ cuts' hd).
+  Proof.
+    remember (Failed _) as f eqn:Hf => + HA.
+    elim: HA B Hf l; clear => //.
+    - move=> s A B HA _ [<-] l vA.
+      rewrite (expand_failure_state_to_list_same HA); auto.
+    - move=> s s' r A B b HA HB IH C ? l vA; subst.
+      have [y [ys [H1 H2]]]:= expand_cb_state_to_list1 l vA HA.
+      have := IH _ erefl l (valid_state_expand vA HA).
+      rewrite !(H1 l).
+      move=>[].
+        admit.
+      move=> [hd[p[t[tl[gl [[??]H]]]]]]; subst.
+      right; repeat eexists.
+        rewrite -cat_cons//.
+      move=>//.
+    - admit.
+  Admitted.
+
+  (* if the s2l of C has a non empty head, then the state is made
+      by some Bot that are going to be canceled by next_alt *)
+  Lemma next_alt_s2l_cons {s1 C s3 D x xs tl l1}:
+    valid_state C ->
+    next_alt s1 C = Some (s3, D) ->
+      state_to_list C l1 = (x :: xs) :: tl -> 
+        state_to_list C l1 = state_to_list D l1.
+  Proof.
+    elim: C s1 s3 D x xs tl l1 => //.
+    - move=> p [|t]//=???????? [_<-][???]; subst => //.
+    - move=> A HA s B HB s1 s2 C x xs tl l1/=.
+      case: ifP => [dA vB|dA /andP[vA bB]].
+        case nB: next_alt => [[s3 D]|]//[??]; subst => /=.
+        rewrite state_to_list_dead//=.
+        rewrite (state_to_list_dead dA)//=.
+        case sB: state_to_list => [|[|z zs] ws]//.
+        have:= HB _ _ _ _ _ _ _ vB nB sB.
+        rewrite sB => <-//.
+      case nA: next_alt => [[s3 D]|].
+        move=>[_<-]/=; case sA: state_to_list => //=[|y ys].
+          by rewrite (state_to_list_empty_next_alt vA sA) in nA.
+        case: y sA => //[z zs] sA/=.
+        have:= HA _ _ _ _ _ _ _ vA nA sA.
+        rewrite sA.
+        case sD: state_to_list => [|[|t ts] rs]//[???]; subst => /=.
+        move=>//.
+      have vB:= bbOr_valid bB.
+      rewrite (valid_state_dead1 vB).
+      move: bB;rewrite /bbOr=> /orP[]; last first.
+        move=>/next_alt_aux_base_or_ko->//.
+      case nB: next_alt => [[w ws]|]//bB.
+      have H := base_or_aux_next_alt_some bB nB.
+      move=>[_<-]/=; rewrite (state_to_list_dead is_dead_dead)/=.
+      rewrite H.
+      have [r [H1 H2]]:= next_alt_none_s2l ((state_to_list ws l1 ++ l1)) vA nA.
+      rewrite H1 incr_cuts_cat.
+      case: r H1 H2 => [|[|m ms] rs]//.
+    - move=> A HA B0 _ B HB s1 s2 C x xs tl l1/= /and5P[oA vA aB].
+      case:(ifP (is_dead _)) => //dA.
+      case:ifP => /=[sA vB bB0|sA /eqP->].
+        rewrite success_failed//=.
+        rewrite success_state_to_list// add_alt_empty1.
+        case nB: next_alt => [[w ws]|]//.
+          move=>[??]; subst =>/=.
+          rewrite (success_state_to_list sA)// !add_alt_empty1.
+          case sB: state_to_list => [|c cs].
+            rewrite (state_to_list_empty_next_alt _ sB)// in nB.
+          case: c sB => //d ds sB.
+          have:= HB _ _ _ _ _ _ _ vB nB sB.
+          move=><-; rewrite sB//.
+        case nA: next_alt => //[[s3 D]].
+        case: ifP => //fB0[??]; subst => /=.
+        move: bB0; rewrite/bbAnd => /orP[]; last first.
+          move=>/base_and_ko_failed; rewrite fB0//.
+        move=>/[dup]/base_and_state_to_list[hd H] bB0.
+        have [r [H1 H2]]:= next_alt_none_s2l l1 vB nB.
+        rewrite H H1; subst.
+        have H1:= clean_successP vA sA nA.
+        rewrite H1.
+        case scA : (state_to_list (clean_success _)) => [|c cs].
+          rewrite make_lB0_empty1 make_lB_empty2 cats0 => H3.
+          rewrite H3 in H2.
+          destruct x => //.
+        case sB: state_to_list => //[|d ds]; last first.
+          rewrite sB in H2.
+          destruct d => //.
+        rewrite make_lB_empty1/=.
+        rewrite/make_lB0/==>-[+?]; subst.
+        rewrite /add_alt/make_lB/make_lB0/=.
+        move=> H3; f_equal.
+        f_equal.
+        have H4 := base_and_lvlt bB0 (H [::]).
+        rewrite all_lvlt_add_caF//.
+      case: ifP => [fA bB|fA bB].
+        case nA: next_alt => //[[s3 D]].
+        case: ifP => //fB0[??]; subst => /=.
+        have H := failed_next_alt_some_state_to_list vA fA nA.
+        rewrite H//.
+      rewrite next_alt_aux_base_and// => -[_<-]//.
+  Qed.
+
+  Lemma gtititigi {s s1 s2 A B C D b1 b2} l1:
+    valid_state A ->
+    expandedb s A (Failed B) b1 -> next_alt s B = Some (s1, C) ->
+      runb s1 C s2 D b2 -> state_to_list A l1 = state_to_list B l1 -> 
+       state_to_list B l1 = state_to_list C l1.
+  Proof.
+    remember (Failed _) as f eqn:Hf => + H.
+    elim: H s1 s2 B C D b2 l1 Hf; clear => //.
+    - move=> s A B H s1 s2 C D E b l1 [<-] vA H1 R H2.
+      rewrite -(expand_failure_state_to_list_same H).
+      apply: expand_failure_next_alt_state_to_list_cons vA H H1.
+    - move=> s1 s2 r A B b1 HA HB _ s3 s4 C D E b2 l1 ? vA HC HD; subst.
+      have [x[tl [H1 H2]]]:= expand_cb_state_to_list1 l1 vA HA.
+      rewrite !H1//.
+      have /= := next_alt_s2l_cons (valid_state_expanded (valid_state_expand vA HA) (ex_intro _ _ HB)) HC.
+      move=> H/esym/H//.
+    - move=> s1 s2 r A B b1 HA HB IH s3 s4 C D E b2 l1 ? vA HC HD; subst.
+      have [ss HH]:= next_alt_some HC s2.      
+  Admitted.
+
 
   Lemma runElpiP: forall A, runElpi A.
   Proof.
@@ -1924,23 +2055,18 @@ Module Nur (U : Unif).
       have [x[xs sA]]:= expandedb_failure_next_alt_state_to_list_cons vA HA HB (state_to_list_state_to_list_cons sC) [::].
       rewrite sA.
       exists x, xs; split => //.
+      have:= expandedb_failure_next_alt_state_to_list_cons1 [::] vA HA.
       (* ci sono due tipi di fallimento, 
         - quelli dovuti a dei bot (che spariscono nel nur), quindi la run lavora di più
         - quelli dovuti a una call senza implementazioni che equivale a fare una FailE
       *)
-      Search next_alt Failed.
-
-      
-
-      Search next_alt Failed.
-      remember (Failed B) as f eqn:Hf.
-      elim: HA s' s2 B C D {b2} Hf vA HB {HC} y ys x xs sA sC H; clear => //.
-      - move=> s A B HA s1 s2 _ C D (*b*) [<-] vA HB (*HC*) y ys x xs sA sC H.
-        admit.
-      - move=> s1 s2 r A B b HA HB IH s4 s5 C D E (*b1*) ? vA HC y ys x xs sA sD H1; subst.
-        have [s6 HC']:= next_alt_some HC s2.
-        admit.
-      - admit.
+      move=>[H1|].
+        have:=gtititigi [::] vA HA HB HC H1.
+        rewrite -H1 sA sC =>-[??]; subst.
+        rewrite (same_subst s s')//.
+      move=>[hd[p[t[tl[gl[]]]]]].
+      rewrite sA => -[??]; subst.
+      admit.
   Admitted.
   Print Assumptions runElpiP.
 
